common/Separation_old.v
@@ -31,7 +31,11 @@
 
 Require Import Setoid Program.Basics.
 Require Import Coqlib Decidableplus.
-Require Import AST Integers Values Memory Events Globalenvs.
+Require Import AST_old Integers Values_old Memory_old Events_old Globalenvs_old.
+
+Section WITHMEM.
+  Existing Instance inject_perm_all.
+  Context `{memory_model_prf: Mem.MemoryModel}.
 
 (** * Assertions about memory *)
 
@@ -49,13 +53,12 @@ notion of splitting a memory state into two disjoint halves).  *)
 Record massert : Type := {
   m_pred : mem -> Prop;
   m_footprint: block -> Z -> Prop;
-  (*SACC:*) m_invar_stack: bool;
-  m_invar: forall m m', m_pred m -> Mem.unchanged_on m_footprint m m'
-                                 -> (*SACC:*) (m_invar_stack = true -> Mem.stack m' = Mem.stack m)
-                                 -> m_pred m';
+  m_invar_weak: bool;
+  m_invar_stack: bool;
+  m_invar: forall m m', m_pred m -> (if m_invar_weak then Mem.strong_unchanged_on else Mem.unchanged_on) m_footprint m m' ->
+                   (m_invar_stack = true -> Mem.stack m' = Mem.stack m) ->
+                   m_pred m';
   m_valid: forall m b ofs, m_pred m -> m_footprint b ofs -> Mem.valid_block m b
-  (*SACC:*)
-  (* m_invar_weak : bool; *)
 }.
 
 Notation "m |= p" := (m_pred p m) (at level 74, no associativity) : sep_scope.
@@ -63,10 +66,9 @@ Notation "m |= p" := (m_pred p m) (at level 74, no associativity) : sep_scope.
 (** Implication and logical equivalence between memory predicates *)
 
 Definition massert_imp (P Q: massert) : Prop :=
-  (forall m, m_pred P m -> m_pred Q m) /\ 
-  (forall b ofs, m_footprint Q b ofs -> m_footprint P b ofs) /\
-  (*SACC:*)(*(m_invar_weak Q = true -> m_invar_weak P = true) /\*)
-  (*SACC:*)  (m_invar_stack Q = true -> m_invar_stack P = true).
+  (m_invar_weak Q = true -> m_invar_weak P = true) /\
+  (m_invar_stack Q = true -> m_invar_stack P = true) /\
+  (forall m, m_pred P m -> m_pred Q m) /\ (forall b ofs, m_footprint Q b ofs -> m_footprint P b ofs).
 Definition massert_eqv (P Q: massert) : Prop :=
   massert_imp P Q /\ massert_imp Q P.
 
@@ -77,48 +79,48 @@ Qed.
 
 Remark massert_imp_trans: forall p q r, massert_imp p q -> massert_imp q r -> massert_imp p r.
 Proof.
-  unfold massert_imp; intros; firstorder auto.
+  unfold massert_imp; clear; intros; firstorder auto.
 Qed.
 
 Remark massert_eqv_refl: forall p, massert_eqv p p.
 Proof.
-  unfold massert_eqv, massert_imp; intros. tauto.
+  unfold massert_eqv, massert_imp; clear; intros. tauto.
 Qed.
 
 Remark massert_eqv_sym: forall p q, massert_eqv p q -> massert_eqv q p.
 Proof.
-  unfold massert_eqv, massert_imp; intros. tauto.
+  unfold massert_eqv, massert_imp; clear; intros. tauto.
 Qed.
 
 Remark massert_eqv_trans: forall p q r, massert_eqv p q -> massert_eqv q r -> massert_eqv p r.
 Proof.
-  unfold massert_eqv, massert_imp; intros. firstorder auto. 
+  unfold massert_eqv, massert_imp; clear; intros. firstorder auto.
 Qed.
 
 (** Record [massert_eqv] and [massert_imp] as relations so that they can be used by rewriting tactics. *)
-(*SACC:*Global*) Add Relation massert massert_imp
+Global Add Relation massert massert_imp
   reflexivity proved by massert_imp_refl
   transitivity proved by massert_imp_trans
 as massert_imp_prel.
 
-(*SACC:*Global*) Add Relation massert massert_eqv
+Global Add Relation massert massert_eqv
   reflexivity proved by massert_eqv_refl
   symmetry proved by massert_eqv_sym
   transitivity proved by massert_eqv_trans
 as massert_eqv_prel.
 
-(*SACC:*Global*) Add Morphism m_pred
+Global Add Morphism m_pred
   with signature massert_imp ==> eq ==> impl
   as m_pred_morph_1.
 Proof.
-  intros P Q [A B]. auto.
+  intros P Q [? [A [B C]]]. auto.
 Qed.
 
-(*SACC:*Global*) Add Morphism m_pred
+Global Add Morphism m_pred
   with signature massert_eqv ==> eq ==> iff
   as m_pred_morph_2.
 Proof.
-  intros P Q [[A B] [C D]]. split; auto.
+  intros P Q [[? [A [B B']]] [? [C [D D']]]]. split; auto.
 Qed.
 
 Hint Resolve massert_imp_refl massert_eqv_refl.
@@ -131,34 +133,44 @@ Definition disjoint_footprint (P Q: massert) : Prop :=
 Program Definition sepconj (P Q: massert) : massert := {|
   m_pred := fun m => m_pred P m /\ m_pred Q m /\ disjoint_footprint P Q;
   m_footprint := fun b ofs => m_footprint P b ofs \/ m_footprint Q b ofs;
-(*SACC:*  m_invar_weak := m_invar_weak P || m_invar_weak Q;*)
+  m_invar_weak := m_invar_weak P || m_invar_weak Q;
   m_invar_stack := m_invar_stack P || m_invar_stack Q
 |}.
 Next Obligation.
   repeat split; auto.
   + apply (m_invar P) with m; auto.
-    - eapply Mem.unchanged_on_implies; eauto. simpl; auto.
+    destruct (m_invar_weak P); simpl in *.
+    - eapply Mem.strong_unchanged_on_implies; eauto. simpl; auto.
+    - destruct (m_invar_weak Q).
+      * eapply Mem.strong_unchanged_on_weak.
+        eapply Mem.strong_unchanged_on_implies; eauto. simpl; auto.
+      * eapply Mem.unchanged_on_implies; eauto. simpl; auto.
     - intro A; rewrite A in H1; apply H1. reflexivity.
   + apply (m_invar Q) with m; auto.
-    - eapply Mem.unchanged_on_implies; eauto. simpl; auto.
+    destruct (m_invar_weak Q); try rewrite orb_true_r in *.
+    - eapply Mem.strong_unchanged_on_implies; eauto. simpl; auto.
+    - destruct (m_invar_weak P); simpl in *.
+      * eapply Mem.strong_unchanged_on_weak.
+        eapply Mem.strong_unchanged_on_implies; eauto. simpl; auto.
+      * eapply Mem.unchanged_on_implies; eauto. simpl; auto.
     - intro A; rewrite A in H1; apply H1. rewrite orb_true_r. reflexivity.
 Qed.
 Next Obligation.
   destruct H0; [eapply (m_valid P) | eapply (m_valid Q)]; eauto.
 Qed.
 
-(*SACC:*Global*) Add Morphism sepconj
+Global Add Morphism sepconj
   with signature massert_imp ==> massert_imp ==> massert_imp
   as sepconj_morph_1.
 Proof.
-  intros P1 P2 [I [B A]] Q1 Q2 [J [D C]].
+  intros P1 P2 [I [A B]] Q1 Q2 [J [C D]].
   red; simpl; split; [ | split ] ; intros.
-  - intuition auto. red; intros. apply (H2 b ofs); auto. 
-  - intuition auto.
   - rewrite Bool.orb_true_iff in * |- * . tauto.
+  - rewrite Bool.orb_true_iff in * |- * . tauto.
+  - intuition auto. red; intros. apply (H6 b ofs); auto. 
 Qed.
 
-(*SACC:*Global*) Add Morphism sepconj
+Global Add Morphism sepconj
   with signature massert_eqv ==> massert_eqv ==> massert_eqv
   as sepconj_morph_2.
 Proof.
@@ -179,9 +191,10 @@ Qed.
 Lemma sep_comm_1:
   forall P Q,  massert_imp (P ** Q) (Q ** P).
 Proof.
-  unfold massert_imp; simpl; split; intros.
-- intuition auto. red; intros; eapply H2; eauto.
-- intuition auto. rewrite Bool.orb_true_iff in * |- * . tauto.
+  unfold massert_imp; simpl; split; [ | split] ; intros.
+  - rewrite Bool.orb_true_iff in * |- * . tauto.
+  - rewrite Bool.orb_true_iff in * |- * . tauto.
+  - intuition auto. red; intros; eapply H2; eauto.
 Qed.
 
 Lemma sep_comm:
@@ -195,14 +208,16 @@ Lemma sep_assoc_1:
 Proof.
   intros. unfold massert_imp, sepconj, disjoint_footprint; simpl. clear. firstorder auto.
   repeat rewrite Bool.orb_true_iff in * |- * ; tauto.
+  repeat rewrite Bool.orb_true_iff in * |- * ; tauto.
 Qed.
 
 Lemma sep_assoc_2:
   forall P Q R, massert_imp (P ** (Q ** R)) ((P ** Q) ** R).
 Proof.
-  intros. unfold massert_imp, sepconj, disjoint_footprint; simpl; firstorder auto.
+  intros. unfold massert_imp, sepconj, disjoint_footprint; simpl; clear; firstorder auto.
   repeat rewrite Bool.orb_true_iff in * |- * ; tauto.
-Qed.  
+  repeat rewrite Bool.orb_true_iff in * |- * ; tauto.
+Qed.
 
 Lemma sep_assoc:
   forall P Q R, massert_eqv ((P ** Q) ** R) (P ** (Q ** R)).
@@ -320,9 +335,9 @@ Qed.
 
 Program Definition pure (P: Prop) : massert := {|
   m_pred := fun m => P;
-(*SACC:*)m_invar_stack := false;
-(*SACC:*)(*m_invar_weak := false;*)
-  m_footprint := fun b ofs => False
+  m_footprint := fun b ofs => False;
+  m_invar_weak := false;
+  m_invar_stack := false;
 |}.
 Next Obligation.
   tauto.
@@ -337,12 +352,13 @@ Qed.
 (** A range of bytes, with full permissions and unspecified contents. *)
 
 Program Definition range (b: block) (lo hi: Z) : massert := {|
-  (*SACC:*)(*m_invar_weak := false  ;*)
-  (*SACC:*)m_invar_stack := false;
   m_pred := fun m =>
        0 <= lo /\ hi <= Ptrofs.modulus
-    /\ (forall i k p, lo <= i < hi -> Mem.perm m b i k p);
+       /\ (forall i k p, lo <= i < hi -> Mem.perm m b i k p);
   m_footprint := fun b' ofs' => b' = b /\ lo <= ofs' < hi
+  ;
+  m_invar_weak := false  ;
+  m_invar_stack := false
 |}.
 Next Obligation.
   split; auto. split; auto. intros. eapply Mem.perm_unchanged_on; eauto. simpl; auto.
@@ -356,15 +372,19 @@ Lemma alloc_rule:
   Mem.alloc m lo hi = (m', b) ->
   0 <= lo -> hi <= Ptrofs.modulus ->
   m |= P ->
+  m_invar_stack P = false ->
   m' |= range b lo hi ** P.
 Proof.
   intros; simpl. split; [|split]. 
 - split; auto. split; auto. intros.
   apply Mem.perm_implies with Freeable; auto with mem.
   eapply Mem.perm_alloc_2; eauto.
-- apply (m_invar P) with m; auto. eapply Mem.alloc_unchanged_on; eauto.
-  intros. eapply Mem.alloc_stack_unchanged. apply H.
-- red; simpl. intros. destruct H3; subst b0.
+- apply (m_invar P) with m; auto.
+  destruct (m_invar_weak P).
+  + eapply Mem.alloc_strong_unchanged_on; eauto.
+  + eapply Mem.alloc_unchanged_on; eauto.
+  + congruence.
+- red; simpl. intros. destruct H4; subst b0.
   eelim Mem.fresh_block_alloc; eauto. eapply (m_valid P); eauto.
 Qed.
 
@@ -375,14 +395,12 @@ Lemma range_split:
   m |= range b lo mid ** range b mid hi ** P.
 Proof.
   intros. rewrite <- sep_assoc. eapply sep_imp; eauto. 
-  split; simpl; intros.
-- intuition auto.
-+ omega.
-+ apply H5; omega.
-+ omega.
-+ apply H5; omega.
-+ red; simpl; intros; omega.
-- intuition omega.
+  split; [ | split; [|split]]; simpl; intros; try assumption.
+  - intuition auto; try omega.
+    + apply H5; omega.
+    + apply H5; omega.
+    + red; simpl; intros; omega.
+  - intuition omega.
 Qed.
 
 Lemma range_drop_left:
@@ -405,21 +423,17 @@ Qed.
 
 Lemma range_split_2:
   forall b lo hi P mid al m,
-  lo <= align mid al <= hi ->
-  al > 0 ->
-  m |= range b lo hi ** P ->
-  m |= range b lo mid ** range b (align mid al) hi ** P.
+    lo <= align mid al <= hi ->
+    al > 0 ->
+    m |= range b lo hi ** P ->
+    m |= range b lo mid ** range b (align mid al) hi ** P.
 Proof.
   intros. rewrite <- sep_assoc. eapply sep_imp; eauto.
   assert (mid <= align mid al) by (apply align_le; auto).
-  split; simpl; intros.
-- intuition auto.
-+ omega.
-+ apply H7; omega.
-+ omega.
-+ apply H7; omega.
-+ red; simpl; intros; omega.
-- intuition omega.
+  split; [ | split; [ | split ] ] ; simpl; intros; try assumption.
+  - intuition auto; try (apply H7; omega); try omega.
+    red; simpl; intros; omega.
+  - intuition omega.
 Qed.
 
 Lemma range_preserved:
@@ -434,18 +448,21 @@ Qed.
 (** A memory area that contains a value sastifying a given predicate *)
 
 Program Definition contains (chunk: memory_chunk) (b: block) (ofs: Z) (spec: val -> Prop) : massert := {|
-(*SACC:*)(*m_invar_weak := false;*)
-(*SACC:*)m_invar_stack := false;
   m_pred := fun m =>
        0 <= ofs <= Ptrofs.max_unsigned
-    /\ Mem.valid_access m chunk b ofs Freeable (*SACC: comment this*)
-(*SACC:*)(*/\  Mem.range_perm m b ofs (ofs + size_chunk chunk) Cur Freeable*)
-    /\ exists v, Mem.load chunk m b ofs = Some v /\ spec v;
+       (* /\ (Mem.valid_access m chunk b ofs Freeable) *)
+       /\  Mem.range_perm m b ofs (ofs + size_chunk chunk) Cur Freeable
+       /\ (align_chunk chunk | ofs)
+       /\ exists v, Mem.load chunk m b ofs = Some v /\ spec v;
   m_footprint := fun b' ofs' => b' = b /\ ofs <= ofs' < ofs + size_chunk chunk
+  ;
+  m_invar_weak := false
+  ;
+  m_invar_stack := false
 |}.
 Next Obligation.
-  rename H3 into v. split;[|split]; auto.
-- destruct H2; split; auto. red; intros; eapply Mem.perm_unchanged_on; eauto. simpl; auto.
+  rename H4 into v. split;[|split;[|split]]; auto.
+- red; intros; eapply Mem.perm_unchanged_on; eauto. simpl; auto.
 - exists v. split; auto. eapply Mem.load_unchanged_on; eauto. simpl; auto.
 Qed.
 Next Obligation.
@@ -465,7 +482,7 @@ Lemma load_rule:
   m |= contains chunk b ofs spec ->
   exists v, Mem.load chunk m b ofs = Some v /\ spec v.
 Proof.
-  intros. destruct H as (D & E & v & F & G).
+  intros. destruct H as (D & E & AL & v & F & G).
   exists v; auto.
 Qed.
 
@@ -480,26 +497,39 @@ Qed.
 
 Lemma store_rule:
   forall chunk m b ofs v (spec1 spec: val -> Prop) P,
-  m |= contains chunk b ofs spec1 ** P ->
+    m |= contains chunk b ofs spec1 ** P ->
+    stack_access (Mem.stack m) b ofs (ofs + size_chunk chunk) ->
   spec (Val.load_result chunk v) ->
   exists m',
   Mem.store chunk m b ofs v = Some m' /\ m' |= contains chunk b ofs spec ** P.
 Proof.
   intros. destruct H as (A & B & C). destruct A as (D & E & v0 & F & G).
-  assert (H: Mem.valid_access m chunk b ofs Writable) by eauto with mem.
-  destruct (Mem.valid_access_store _ _ _ _ v H) as [m' STORE].
+  assert (H: Mem.valid_access m chunk b ofs Freeable).
+  {
+    split;[|split]; eauto.
+  }
+  assert (H2: Mem.valid_access m chunk b ofs Writable).
+  {
+    eauto with mem.
+  }
+  destruct (Mem.valid_access_store _ _ _ _ v H2) as [m' STORE].
   exists m'; split; auto. simpl. intuition auto.
 - eapply Mem.store_valid_access_1; eauto.
 - exists (Val.load_result chunk v); split; auto. eapply Mem.load_store_same; eauto. 
 - apply (m_invar P) with m; auto. 
-  eapply Mem.store_unchanged_on; eauto. 
-  intros; red; intros. apply (C b i); simpl; auto. 
-  intros; eapply Mem.store_stack_unchanged; eauto.
+  destruct (m_invar_weak P).
+  + eapply Mem.store_strong_unchanged_on; eauto.
+    intros; red; intros. apply (C b i); simpl; auto.
+  + eapply Mem.store_unchanged_on; eauto.
+    intros; red; intros. apply (C b i); simpl; auto.
+  + intros.
+    eapply Mem.store_stack_blocks; eauto.
 Qed.
 
 Lemma storev_rule:
   forall chunk m b ofs v (spec1 spec: val -> Prop) P,
-  m |= contains chunk b ofs spec1 ** P ->
+    m |= contains chunk b ofs spec1 ** P ->
+    stack_access (Mem.stack m) b ofs (ofs + size_chunk chunk) ->
   spec (Val.load_result chunk v) ->
   exists m',
   Mem.storev chunk m (Vptr b (Ptrofs.repr ofs)) v = Some m' /\ m' |= contains chunk b ofs spec ** P.
@@ -512,6 +542,7 @@ Lemma range_contains:
   forall chunk b ofs P m,
   m |= range b ofs (ofs + size_chunk chunk) ** P ->
   (align_chunk chunk | ofs) ->
+  stack_access (Mem.stack m) b ofs (ofs + size_chunk chunk) ->
   m |= contains chunk b ofs (fun v => True) ** P.
 Proof.
   intros. destruct H as (A & B & C). destruct A as (D & E & F).
@@ -519,8 +550,9 @@ Proof.
 - assert (Mem.valid_access m chunk b ofs Freeable).
   { split; auto. red; auto. }
   split. generalize (size_chunk_pos chunk). unfold Ptrofs.max_unsigned. omega.
-  split. auto.
-+ destruct (Mem.valid_access_load m chunk b ofs) as [v LOAD].
+  split; [|split]; auto.
+  apply H.
+  destruct (Mem.valid_access_load m chunk b ofs) as [v LOAD].
   eauto with mem.
   exists v; auto.
 - auto.
@@ -532,35 +564,32 @@ Lemma contains_imp:
   (forall v, spec1 v -> spec2 v) ->
   massert_imp (contains chunk b ofs spec1) (contains chunk b ofs spec2).
 Proof.
-  intros; split; simpl; intros.
-- intuition auto. destruct H4 as (v & A & B). exists v; auto.
-- auto.
+  intros; split; [| split; [ | split ]] ; simpl; intros.
+  - assumption.
+  - assumption.
+  - intuition auto. destruct H5 as (v & A & B). exists v; auto.
+  - auto.
 Qed.
 
-(*SACC:*)
-(*
-Program Definition contains_ra (chunk: memory_chunk) (b: block) (ofs: Z) (ra: val) : massert := {|
-(*SACC:*)(*m_invar_weak := false;*)
-(*SACC:*)m_invar_stack := false;
+Program Definition contains_ra (b: block) (ofs: Z) (ra: val) : massert := {|
   m_pred := fun m =>
        0 <= ofs <= Ptrofs.max_unsigned
-    /\ Mem.valid_access m Mptr b ofs Freeable (*SACC: comment this*)
-(*SACC:*)(*/\  Mem.range_perm m b ofs (ofs + size_chunk chunk) Cur Freeable*)
-    /\ Mem.loadbytesv Mptr m (Vptr b (Ptrofs.repr ofs)) = Some ra;
-  m_footprint := fun b' ofs' => b' = b /\ ofs <= ofs' < ofs + size_chunk Mptr
+       /\  Mem.range_perm m b ofs (ofs + size_chunk Mptr) Cur Freeable
+       /\ (align_chunk Mptr | ofs)
+       /\ Mem.loadbytesv Mptr m (Vptr b (Ptrofs.repr ofs)) = Some ra;
+  m_footprint := fun b' ofs' => b' = b /\ ofs <= ofs' < ofs + size_chunk Mptr;
+  m_invar_weak := false;
+  m_invar_stack := false;
 |}.
 Next Obligation.
-  destr_in H3. clear H1.
-  repeat apply conj; auto;
-  destruct H2; eauto.
+  destr_in H4. clear H1.
+  repeat apply conj; auto.
 - red; intros; eapply Mem.perm_unchanged_on; eauto. simpl; auto.
-- erewrite Mem.loadbytes_unchanged_on; eauto.  simpl.  
-  rewrite Ptrofs.unsigned_repr by omega. auto.
+- erewrite Mem.loadbytes_unchanged_on; eauto.  simpl.  rewrite Ptrofs.unsigned_repr by omega. auto. 
 Qed.
 Next Obligation.
   eauto with mem. 
 Qed. 
-*)
 
 (** A memory area that contains a given value *)
 
@@ -569,8 +598,9 @@ Definition hasvalue (chunk: memory_chunk) (b: block) (ofs: Z) (v: val) : massert
 
 Lemma store_rule':
   forall chunk m b ofs v (spec1: val -> Prop) P,
-  m |= contains chunk b ofs spec1 ** P ->
-  exists m',
+    m |= contains chunk b ofs spec1 ** P ->
+    stack_access (Mem.stack m) b ofs (ofs + size_chunk chunk) ->
+    exists m',
   Mem.store chunk m b ofs v = Some m' /\ m' |= hasvalue chunk b ofs (Val.load_result chunk v) ** P.
 Proof.
   intros. eapply store_rule; eauto. 
@@ -578,9 +608,10 @@ Qed.
 
 Lemma storev_rule':
   forall chunk m b ofs v (spec1: val -> Prop) P,
-  m |= contains chunk b ofs spec1 ** P ->
-  exists m',
-  Mem.storev chunk m (Vptr b (Ptrofs.repr ofs)) v = Some m' /\ m' |= hasvalue chunk b ofs (Val.load_result chunk v) ** P.
+    m |= contains chunk b ofs spec1 ** P ->
+    stack_access (Mem.stack m) b ofs (ofs + size_chunk chunk) ->
+    exists m',
+      Mem.storev chunk m (Vptr b (Ptrofs.repr ofs)) v = Some m' /\ m' |= hasvalue chunk b ofs (Val.load_result chunk v) ** P.
 Proof.
   intros. eapply storev_rule; eauto.
 Qed.
@@ -588,17 +619,30 @@ Qed.
 (** Non-separating conjunction *)
 
 Program Definition mconj (P Q: massert) : massert := {|
-(*SACC:*)(*m_invar_weak := m_invar_weak P || m_invar_weak Q;*)
-(*SACC:*)  m_invar_stack := m_invar_stack P || m_invar_stack Q;
   m_pred := fun m => m_pred P m /\ m_pred Q m;
   m_footprint := fun b ofs => m_footprint P b ofs \/ m_footprint Q b ofs
+  ;
+  m_invar_weak := m_invar_weak P || m_invar_weak Q;
+  m_invar_stack := m_invar_stack P || m_invar_stack Q;
 |}.
 Next Obligation.
-  split. 
-  apply (m_invar P) with m; auto. eapply Mem.unchanged_on_implies; eauto. simpl; auto.
-  intros; apply H1. rewrite H3. reflexivity.
-  apply (m_invar Q) with m; auto. eapply Mem.unchanged_on_implies; eauto. simpl; auto.
-  intros; apply H1. rewrite H3, orb_true_r; reflexivity.
+  repeat split; auto.
+  + apply (m_invar P) with m; auto.
+    destruct (m_invar_weak P); simpl in *.
+    - eapply Mem.strong_unchanged_on_implies; eauto. simpl; auto.
+    - destruct (m_invar_weak Q).
+      * apply Mem.strong_unchanged_on_weak.
+        eapply Mem.strong_unchanged_on_implies; eauto. simpl; auto.
+      * eapply Mem.unchanged_on_implies; eauto. simpl; auto.
+    - intros; apply H1. rewrite H3; reflexivity.        
+  + apply (m_invar Q) with m; auto.
+    destruct (m_invar_weak Q); try rewrite orb_true_r in *.
+    - eapply Mem.strong_unchanged_on_implies; eauto. simpl; auto.
+    - destruct (m_invar_weak P); simpl in *.
+      * apply Mem.strong_unchanged_on_weak.
+        eapply Mem.strong_unchanged_on_implies; eauto. simpl; auto.
+      * eapply Mem.unchanged_on_implies; eauto. simpl; auto.
+    - intros; apply H1. rewrite H3, orb_true_r; reflexivity.
 Qed.
 Next Obligation.
   destruct H0; [eapply (m_valid P) | eapply (m_valid Q)]; eauto.
@@ -644,16 +688,17 @@ Proof.
   red; simpl; intros. destruct H2. eapply F; eauto. eapply C; simpl; eauto.
 Qed.
 
-(*SACC:*Global*) Add Morphism mconj
+Global Add Morphism mconj
   with signature massert_imp ==> massert_imp ==> massert_imp
   as mconj_morph_1.
 Proof.
-  intros P1 P2 [A B] Q1 Q2 [C D].
+  intros P1 P2 [I [A B]] Q1 Q2 [J [C D]].
   red; simpl; intuition auto.
+  repeat rewrite Bool.orb_true_iff in * |- * . tauto.
   repeat rewrite Bool.orb_true_iff in * |- * . tauto.
 Qed.
 
-(*SACC:*Global*) Add Morphism mconj
+Global Add Morphism mconj
   with signature massert_eqv ==> massert_eqv ==> massert_eqv
   as mconj_morph_2.
 Proof.
@@ -663,13 +708,13 @@ Qed.
 (** The image of a memory injection *)
 
 Program Definition minjection (j: meminj) g (m0: mem) : massert := {|
-(*SACC:*) m_invar_stack := true;
-(*SACC:*)(*m_invar_weak := true;*)
   m_pred := fun m => Mem.inject j g m0 m;
-  m_footprint := fun b ofs => exists b0 delta, j b0 = Some(b, delta) /\ Mem.perm m0 b0 (ofs - delta) Max Nonempty
+  m_footprint := fun b ofs => exists b0 delta, j b0 = Some(b, delta) /\ Mem.perm m0 b0 (ofs - delta) Max Nonempty;
+  m_invar_weak := true;
+  m_invar_stack := true;
 |}.
 Next Obligation.
-  eapply Mem.inject_unchanged_on; eauto.
+  eapply Mem.inject_strong_unchanged_on; eauto.
 Qed.
 Next Obligation.
   eapply Mem.valid_block_inject_2; eauto.
@@ -704,31 +749,35 @@ Proof.
   split; [|split].
 - exact INJ.
 - apply (m_invar P) with m2; auto.
-  eapply Mem.store_unchanged_on; eauto.
+  cut (Mem.strong_unchanged_on (m_footprint P) m2 m2').
+  {
+    destruct (m_invar_weak P); auto using Mem.strong_unchanged_on_weak.
+  }
+  eapply Mem.store_strong_unchanged_on; eauto.
   intros; red; intros. eelim C; eauto. simpl.
   exists b1, delta; split; auto. destruct VALID as [V1 V2]. 
   apply Mem.perm_cur_max. apply Mem.perm_implies with Writable; auto with mem. 
   apply V1. omega.
-  intros. eapply Mem.store_stack_unchanged. apply STORE.
+  intros; eapply Mem.store_stack_blocks; eauto.
 - red; simpl; intros. destruct H1 as (b0 & delta0 & U & V).
   eelim C; eauto. simpl. exists b0, delta0; eauto with mem.
 Qed.
 
 Lemma alloc_parallel_rule:
   forall m1 sz1 m1' b1 m2 sz2 m2' b2 P j g lo hi delta,
-  m2 |= minjection j g m1 ** P ->
-  Mem.alloc m1 0 sz1 = (m1', b1) ->
-  Mem.alloc m2 0 sz2 = (m2', b2) ->
-  (8 | delta) ->
-  lo = delta ->
-  hi = delta + Zmax 0 sz1 ->
-  0 <= sz2 <= Ptrofs.max_unsigned ->
-  0 <= delta -> hi <= sz2 ->
-  exists j',
-     m2' |= range b2 0 lo ** range b2 hi sz2 ** minjection j' g m1' ** P
-  /\ inject_incr j j'
-  /\ j' b1 = Some(b2, delta)
-  /\ (forall b, b <> b1 -> j' b = j b).
+    m2 |= minjection j g m1 ** P ->
+    Mem.alloc m1 0 sz1 = (m1', b1) ->
+    Mem.alloc m2 0 sz2 = (m2', b2) ->
+    (8 | delta) ->
+    lo = delta ->
+    hi = delta + Zmax 0 sz1 ->
+    0 <= sz2 <= Ptrofs.max_unsigned ->
+    0 <= delta -> hi <= sz2 ->
+    exists j',
+      m2' |= range b2 0 lo ** range b2 hi sz2 ** minjection j' g m1' ** P
+      /\ inject_incr j j'
+      /\ j' b1 = Some(b2, delta)
+      /\ (forall b, b <> b1 -> j' b = j b).
 Proof.
   intros until delta; intros SEP ALLOC1 ALLOC2 ALIGN LO HI RANGE1 RANGE2 RANGE3.
   assert (RANGE4: lo <= hi) by xomega.
@@ -736,51 +785,61 @@ Proof.
   assert (FRESH2: ~Mem.valid_block m2 b2) by (eapply Mem.fresh_block_alloc; eauto).
   destruct SEP as (INJ & SP & DISJ). simpl in INJ.
   exploit Mem.alloc_left_mapped_inject.
-- eapply Mem.alloc_right_inject; eauto. 
-- eexact ALLOC1.
-- instantiate (1 := b2). eauto with mem.
-- instantiate (1 := delta). xomega.
-- intros. assert (0 <= ofs < sz2) by (eapply Mem.perm_alloc_3; eauto). omega.
-- intros. apply Mem.perm_implies with Freeable; auto with mem. 
-  eapply Mem.perm_alloc_2; eauto. xomega.
-- red; intros. apply Zdivides_trans with 8; auto. 
-  exists (8 / align_chunk chunk). destruct chunk; reflexivity.
-- intros. elim FRESH2. eapply Mem.valid_block_inject_2; eauto. 
-- intros (j' & INJ' & J1 & J2 & J3).
-  exists j'; split; auto.
-  rewrite <- ! sep_assoc.
-  split; [|split].
-+ simpl. intuition auto; try (unfold Ptrofs.max_unsigned in *; omega).
-* apply Mem.perm_implies with Freeable; auto with mem.
-  eapply Mem.perm_alloc_2; eauto. omega. 
-* apply Mem.perm_implies with Freeable; auto with mem.
-  eapply Mem.perm_alloc_2; eauto. omega. 
-* red; simpl; intros. destruct H1, H2. omega.
-* red; simpl; intros.
-  assert (b = b2) by tauto. subst b.
-  assert (0 <= ofs < lo \/ hi <= ofs < sz2) by tauto. clear H1.
-  destruct H2 as (b0 & delta0 & D & E).
-  eapply Mem.perm_alloc_inv in E; eauto. 
-  destruct (eq_block b0 b1).
-  subst b0. rewrite J2 in D. inversion D; clear D; subst delta0. xomega.
-  rewrite J3 in D by auto. elim FRESH2. eapply Mem.valid_block_inject_2; eauto. 
-+ apply (m_invar P) with m2; auto. eapply Mem.alloc_unchanged_on; eauto.
-  intros. eapply Mem.alloc_stack_unchanged. apply ALLOC2.
-+ red; simpl; intros.
-  assert (VALID: Mem.valid_block m2 b) by (eapply (m_valid P); eauto).
-  destruct H as [A | (b0 & delta0 & A & B)].
-* assert (b = b2) by tauto. subst b. contradiction.
-* eelim DISJ; eauto. simpl. 
-  eapply Mem.perm_alloc_inv in B; eauto. 
-  destruct (eq_block b0 b1).
-  subst b0. rewrite J2 in A. inversion A; clear A; subst b delta0. contradiction.
-  rewrite J3 in A by auto. exists b0, delta0; auto.
+  - eapply Mem.alloc_right_inject; eauto. 
+  - eexact ALLOC1.
+  - instantiate (1 := b2). eauto with mem.
+  - instantiate (1 := delta). xomega.
+  - intros. assert (0 <= ofs < sz2) by (eapply Mem.perm_alloc_3; eauto). omega.
+  - intros. apply Mem.perm_implies with Freeable; auto with mem. 
+    eapply Mem.perm_alloc_2; eauto. xomega.
+  - red; intros. apply Zdivides_trans with 8; auto. 
+    exists (8 / align_chunk chunk). destruct chunk; reflexivity.
+  - intros. elim FRESH2. eapply Mem.valid_block_inject_2; eauto.
+  - intros fi IFS o k pp PERM IPC. erewrite Mem.alloc_stack_blocks in IFS. 2: eauto.
+    exfalso; apply FRESH2. apply Mem.in_frames_valid. eapply in_stack'_in_stack; eauto.
+  - intros (j' & INJ' & J1 & J2 & J3).
+    exists j'; split; auto.
+    rewrite <- ! sep_assoc.
+    split; [|split].
+    + simpl. intuition auto; try (unfold Ptrofs.max_unsigned in *; omega).
+      * apply Mem.perm_implies with Freeable; auto with mem.
+        eapply Mem.perm_alloc_2; eauto. omega. 
+      (* * red; right; red; erewrite Mem.alloc_get_frame_info_fresh; eauto. *)
+      * apply Mem.perm_implies with Freeable; auto with mem.
+        eapply Mem.perm_alloc_2; eauto. omega. 
+      (* * red; right; red; erewrite Mem.alloc_get_frame_info_fresh; eauto. *)
+      * red; simpl; intros. destruct H1, H2. omega.
+      * red; simpl; intros.
+        assert (b = b2) by tauto. subst b.
+        assert (0 <= ofs < lo \/ hi <= ofs < sz2) by tauto. clear H1.
+        destruct H2 as (b0 & delta0 & D & E).
+        eapply Mem.perm_alloc_inv in E; eauto. 
+        destruct (eq_block b0 b1).
+        subst b0. rewrite J2 in D. inversion D; clear D; subst delta0. xomega.
+        rewrite J3 in D by auto. elim FRESH2. eapply Mem.valid_block_inject_2; eauto. 
+    + apply (m_invar P) with m2; auto.
+      cut (Mem.strong_unchanged_on (m_footprint P) m2 m2').
+      {
+        destruct (m_invar_weak P); auto using Mem.strong_unchanged_on_weak.
+      }
+      eapply Mem.alloc_strong_unchanged_on; eauto.
+      intros; eapply Mem.alloc_stack_blocks; eauto.
+    + red; simpl; intros.
+      assert (VALID: Mem.valid_block m2 b) by (eapply (m_valid P); eauto).
+      destruct H as [A | (b0 & delta0 & A & B)].
+      * assert (b = b2) by tauto. subst b. contradiction.
+      * eelim DISJ; eauto. simpl. 
+        eapply Mem.perm_alloc_inv in B; eauto. 
+        destruct (eq_block b0 b1).
+        subst b0. rewrite J2 in A. inversion A; clear A; subst b delta0. contradiction.
+        rewrite J3 in A by auto. exists b0, delta0; auto.
 Qed.
 
 Lemma free_parallel_rule:
   forall j g m1 b1 sz1 m1' m2 b2 sz2 lo hi delta P,
   m2 |= range b2 0 lo ** range b2 hi sz2 ** minjection j g m1 ** P ->
   Mem.free m1 b1 0 sz1 = Some m1' ->
+  inject_perm_condition Freeable ->
   j b1 = Some (b2, delta) ->
   lo = delta -> hi = delta + Zmax 0 sz1 ->
   exists m2',
@@ -809,7 +868,7 @@ Proof.
   destruct (zlt (ofs + delta0) lo). intuition auto.
   destruct (zle hi (ofs + delta0)). intuition auto. 
   destruct (eq_block b0 b1).
-* subst b0. rewrite H1 in H; inversion H; clear H; subst delta0.
+* subst b0. rewrite H2 in H; inversion H; clear H; subst delta0.
   eelim (Mem.perm_free_2 m1); eauto. xomega.
 * exploit Mem.mi_no_overlap; eauto. 
   apply Mem.perm_max with k. apply Mem.perm_implies with p; auto with mem. 
@@ -822,15 +881,19 @@ Proof.
   replace (ofs + delta0 - delta0) with ofs by omega.
   apply Mem.perm_max with k. apply Mem.perm_implies with p; auto with mem. 
   eapply Mem.perm_free_3; eauto.
-- apply (m_invar P) with m2; auto. 
-  eapply Mem.free_unchanged_on; eauto. 
+- apply (m_invar P) with m2; auto.
+  cut (Mem.strong_unchanged_on (m_footprint P) m2 m2').
+  {
+    destruct (m_invar_weak P); auto using Mem.strong_unchanged_on_weak.
+  }
+  eapply Mem.free_strong_unchanged_on; eauto.
   intros; red; intros. eelim C; eauto. simpl. 
   destruct (zlt i lo). intuition auto.
   destruct (zle hi i). intuition auto.
   right; exists b1, delta; split; auto. 
   apply Mem.perm_cur_max. apply Mem.perm_implies with Freeable; auto with mem.
-  eapply Mem.free_range_perm; eauto. xomega. 
-  intros. eapply Mem.free_stack_unchanged. apply FREE.
+  eapply Mem.free_range_perm; eauto. xomega.
+  intros; eapply Mem.free_stack_blocks; eauto.
 - red; simpl; intros. eelim C; eauto. 
   simpl. right. destruct H as (b0 & delta0 & U & V). 
   exists b0, delta0; split; auto. 
@@ -848,10 +911,10 @@ Inductive globalenv_preserved {F V: Type} (ge: Genv.t F V) (j: meminj) (bound: b
       (VARINFOS: forall b gv, Genv.find_var_info ge b = Some gv -> Plt b bound).
 
 Program Definition globalenv_inject {F V: Type} (ge: Genv.t F V) (j: meminj) : massert := {|
-(*SACC:*)(*m_invar_weak := false;*)
-(*SACC:*)m_invar_stack := false;
   m_pred := fun m => exists bound, Ple bound (Mem.nextblock m) /\ globalenv_preserved ge j bound;
-  m_footprint := fun b ofs => False
+  m_footprint := fun b ofs => False;
+  m_invar_weak := false;
+  m_invar_stack := false;
 |}.
 Next Obligation.
   rename H into bound. exists bound; split; auto. eapply Ple_trans; eauto. eapply Mem.unchanged_on_nextblock; eauto.
@@ -892,8 +955,15 @@ Proof.
 - eauto.
 Qed.
 
+Context `{external_calls_ops: !ExternalCallsOps mem}.
+Context `{symbols_inject'_instance: !SymbolsInject}.
+Context `{external_calls_props: !ExternalCallsProps mem}.
+Context `{enable_builtins_instance: !EnableBuiltins mem}.
+Context `{external_calls_prf: !ExternalCalls mem}.
+
 Lemma external_call_parallel_rule:
   forall (F V: Type) ef (ge: Genv.t F V) vargs1 m1 t vres1 m1' m2 j g P vargs2,
+  m_invar_weak P = false ->
   external_call ef ge vargs1 m1 t vres1 m1' ->
   m2 |= minjection j g m1 ** globalenv_inject ge j ** P ->
   Val.inject_list j vargs1 vargs2 ->
@@ -904,8 +974,8 @@ Lemma external_call_parallel_rule:
   /\ inject_incr j j'
   /\ inject_separated j j' m1 m2.
 Proof.
-  intros until vargs2; intros CALL SEP ARGS.
-  destruct SEP as (A & B & C). simpl in A. 
+  intros until vargs2; intros INV_STRONG CALL SEP ARGS.
+  destruct SEP as (A & B & C). simpl in A.
   exploit external_call_mem_inject; eauto.
   eapply globalenv_inject_preserves_globals. eapply sep_pick1; eauto.
   intros (j' & vres2 & m2' & CALL' & RES & INJ' & UNCH1 & UNCH2 & INCR & ISEP).
@@ -917,9 +987,10 @@ Proof.
 - exact INJ'.
 - apply m_invar with (m0 := m2).
 + apply globalenv_inject_incr with j m1; auto.
-+ eapply Mem.unchanged_on_implies; eauto.
++ simpl. rewrite INV_STRONG.
+  eapply Mem.unchanged_on_implies; eauto.
   intros; red; intros; red; intros.
-  eelim C; eauto. simpl. exists b0, delta; auto.
+  eelim C; simpl; eauto.
 + symmetry; eapply external_call_stack_blocks; eauto.
 - red; intros. destruct H as (b0 & delta & J' & E).
   destruct (j b0) as [[b' delta'] | ] eqn:J.
@@ -942,8 +1013,8 @@ Lemma alloc_parallel_rule_2:
   exists j',
      m2' |= range b2 0 lo ** range b2 hi sz2 ** minjection j' g m1' ** globalenv_inject ge j' ** P
   /\ inject_incr j j'
-  /\ j' b1 = Some(b2, delta).
-(*SACC:  /\ inject_separated j j' m1 m2 .*)
+  /\ j' b1 = Some(b2, delta)
+  /\ inject_separated j j' m1 m2 .
 Proof.
   intros. 
   set (j1 := fun b => if eq_block b b1 then Some(b2, delta) else j b).
@@ -963,15 +1034,16 @@ Proof.
   rewrite sep_swap4 in A. rewrite sep_swap4. apply globalenv_inject_incr with j1 m1; auto.
 - red; unfold j1; intros. destruct (eq_block b b1). congruence. rewrite D; auto.
 - red; unfold j1; intros. destruct (eq_block b0 b1). congruence. rewrite D in H9 by auto. congruence.
+- split; auto.
+  split; auto.
+  red. intros b0 b3 delta0 H8 H9.
+  destruct (peq b0 b1).
+  + subst.
+    rewrite C in H9. inversion H9. subst delta0 b3.
+    eauto with mem.
+  + rewrite D in H9; congruence.
 Qed.
 
-(*====================================*)
-(*====================================*)
-(*SACC: Stack-aware CompCert addendum *)
-(*====================================*)
-(*====================================*)
-
-(*
 Lemma alloc_parallel_rule_2_flat:
   forall (F V: Type) (ge: Genv.t F V) m1 sz1 m1' b1 m2 sz2 m2' b2 P j lo hi delta,
   m2 |= minjection j (flat_frameinj (length (Mem.stack m1))) m1 ** globalenv_inject ge j ** P ->
@@ -989,7 +1061,7 @@ Lemma alloc_parallel_rule_2_flat:
   /\ inject_separated j j' m1 m2 .
 Proof.
   intros.
-  edestruct alloc_parallel_rule_2 as (j' & SEP & INCR & JNEW); eauto.
+  edestruct alloc_parallel_rule_2 as (j' & SEP & INCR & JNEW & JSEP); eauto.
   exists j'; split; eauto.
   rewrite sep_swap3 in SEP |- *.
   eapply sep_imp; eauto.
@@ -999,7 +1071,6 @@ Proof.
   split; auto.
   repeat rewrite_stack_blocks. auto.
 Qed.
-*)
 
 Lemma record_stack_block_parallel_rule:
   forall m1 m1' m2 j P fi b b' delta n,
@@ -1011,6 +1082,9 @@ Lemma record_stack_block_parallel_rule:
       frame_adt_size fa = Z.max 0 n ->
       Mem.record_stack_blocks m1 fa  = Some m1' ->
       (forall o, 0 <= o < frame_size finone -> Mem.perm m1 b o Cur Writable) ->
+      (forall (ofs : Z) (k : perm_kind) (p : permission),
+       Mem.perm m1 b ofs k p ->
+       frame_public fi (ofs + delta)) ->
     (forall (ofs : Z) (k : perm_kind) (p : permission),
         Mem.perm m2 b' ofs k p -> 0 <= ofs < frame_size fi) ->
     (forall bb delta0, j bb = Some (b', delta0) -> bb = b) ->
@@ -1028,17 +1102,20 @@ Lemma record_stack_block_parallel_rule:
       m2' |= minjection j (flat_frameinj (length (Mem.stack m1'))) m1' ** P.
 Proof.
   intros m1 m1' m2 j P fi b b' delta n FB INVAR MINJ NIN fa finone (* PUB *) fablocks fasize
-         RSB1 PERM0 PERM2 UNIQ fa' fa'eq TTNP SEQ.
+         RSB1 PERM0 PERM1 PERM2 UNIQ fa' fa'eq TTNP SEQ.
   destruct MINJ as (MINJ & PM & DISJ).
   Check Mem.record_push_inject_flat.
-  edestruct (Mem.record_push_inject_flat _ _ _ fa fa' m1' MINJ) as (m2' & RSB2 & MINJ'); simpl in *.
+  edestruct (Mem.record_push_inject_flat _ _ _ MINJ fa fa') as (m2' & RSB2 & MINJ'); simpl in *.
   - setoid_rewrite Forall_forall.  intros. destruct x.  simpl in *.
     rewrite fablocks in H. simpl in H. destruct H; try easy. inv H.
     simpl in *. rewrite FB in H0; inv H0.
     eexists; split; eauto.
     constructor.
-    intros. eapply PERM2. eapply Mem.perm_inject. eauto. eauto. eauto.
-    eapply PERM2.  eapply Mem.perm_inject; eauto.
+    + intros.
+      erewrite PERM1; eauto.
+      red. destr. 
+    + intros. eapply PERM2. eapply Mem.perm_inject. eauto. eauto. eauto.
+      apply inject_perm_condition_writable. constructor.
   - intros. unfold in_frame in H0. subst. simpl in *. destruct H0; try easy. subst. congruence.
   - red; unfold in_frame; simpl. subst; simpl. intros ? [B|[]]. subst. simpl in *; eapply Mem.valid_block_inject_2; eauto. 
   - subst; simpl in *; intros ? ? ? ? ? [B|[]]. inv B. eauto.
@@ -1052,7 +1129,10 @@ Proof.
     split; [|split].
     + simpl in *. auto.  
     + eapply m_invar. eauto.
-      * eapply Mem.record_stack_block_unchanged_on; eauto.
+      * 
+        destruct (m_invar_weak P); eauto using Mem.strong_unchanged_on_weak.
+        eapply Mem.record_stack_block_unchanged_on; eauto.
+        eapply Mem.strong_unchanged_on_weak, Mem.record_stack_block_unchanged_on; eauto.
       * congruence.
     + red; intros. eapply DISJ; eauto.
       simpl in *. decompose [ex and] H.
@@ -1068,6 +1148,9 @@ Lemma record_stack_block_parallel_rule_2:
     forall (NIN: ~ in_stack (Mem.stack m2) b') sz,
       Mem.record_stack_blocks m1 (make_singleton_frame_adt b sz n) = Some m1' ->
       (forall o, 0 <= o < sz -> Mem.perm m1 b o Cur Writable) ->
+      (forall (ofs : Z) (k : perm_kind) (p : permission),
+       Mem.perm m1 b ofs k p ->
+       frame_public fi (ofs + delta)) ->
     (forall (ofs : Z) (k : perm_kind) (p : permission),
         Mem.perm m2 b' ofs k p -> 0 <= ofs < frame_size fi) ->
     (forall bb delta0, j bb = Some (b', delta0) -> bb = b) ->
@@ -1077,10 +1160,10 @@ Lemma record_stack_block_parallel_rule_2:
       Mem.record_stack_blocks m2 (make_singleton_frame_adt' b' fi n) = Some m2' /\
       m2' |= minjection j (flat_frameinj (length (Mem.stack m1'))) m1' ** P.
 Proof.
-  intros m1 m1' m2 j P fi b b' delta n H H0 H1 NIN sz H2 H3 H5 H6 TTNP SEQ.
+  intros m1 m1' m2 j P fi b b' delta n H H0 H1 NIN sz H2 H3 H4 H5 H6 TTNP SEQ.
   edestruct record_stack_block_parallel_rule as (m2' & RSB & INJ); eauto.
   reflexivity. reflexivity.
-  simpl. intros. rewrite Zmax_spec in H4. destr_in H4. omega. eauto.  
+  simpl. intros. rewrite Zmax_spec in H7. destr_in H7. omega. eauto.  
 Qed.
 
 Lemma push_rule:
@@ -1095,7 +1178,7 @@ Proof.
   apply INJ.
   eapply m_invar. eauto.
   generalize (Mem.push_new_stage_unchanged_on (m_footprint P) m2).
-  eauto.
+  destruct (m_invar_weak P); eauto using Mem.strong_unchanged_on_weak.
   congruence.
   red; simpl; intros.
   destruct H0 as (b0 & delta & JB & PERM).
@@ -1104,7 +1187,6 @@ Proof.
   exists b0, delta; split; eauto.
 Qed.
 
-(*SACC:
 Lemma push_rule_2:
   forall j g m1 m2 P Q,
     m2 |= mconj (minjection j g m1) Q ** P ->
@@ -1119,10 +1201,11 @@ Proof.
   eapply sep_imp. apply SEP.
   red; split; auto. split; auto. auto.
   eapply m_invar. apply mconj_proj2 in SEP. apply SEP.
+  destr.
   eapply Mem.push_new_stage_unchanged_on.
+  eapply Mem.strong_unchanged_on_weak, Mem.push_new_stage_unchanged_on.
   simpl. congruence.
 Qed.
-*)
 
 Lemma unrecord_stack_block_parallel_rule:
   forall m1 m1' m2 j g P,
@@ -1141,7 +1224,7 @@ Proof.
   - simpl in *. auto.
   - eapply m_invar. eauto.
     exploit Mem.unrecord_stack_block_unchanged_on. eauto.
-    eauto.
+    destruct (m_invar_weak P); eauto using Mem.strong_unchanged_on_weak.
     congruence.
   - red; intros. eapply DISJ. 2: eauto. simpl in H |- *.
     decompose [ex and] H.
@@ -1149,7 +1232,6 @@ Proof.
     eapply Mem.unrecord_stack_block_perm; eauto.
 Qed.
 
-(*SACC:
 Lemma pop_frame_parallel_rule:
   forall (j : meminj) g (m1 : mem) (b1 : block) (sz1 sz2 : Z) (m1' m1'' m2 : mem) (b2 : block) (lo hi delta n : Z) (P : massert),
     m_invar_stack P = false ->
@@ -1172,4 +1254,11 @@ Proof.
   intros (m2'0 & UNRECORD' & SEP'').
   eexists; eexists; eauto.
 Qed.
-*)
+
+End WITHMEM.
+
+Notation "m |= p" := (m_pred p m) (at level 74, no associativity) : sep_scope.
+
+Hint Resolve massert_imp_refl massert_eqv_refl.
+
+Infix "**" := sepconj (at level 60, right associativity) : sep_scope.
