common/StackADT.v
@@ -6,7 +6,7 @@ Require Import Values.
 Require Export Assoc.
 Require Intv.
 
-Open Scope nat_scope.
+Local Open Scope nat_scope.
 
 (* To be moved to Coqlib *)
 Definition option_prop {A} (P: A -> Prop) (oa: option A): Prop :=
@@ -25,44 +25,6 @@ Definition option_prop2 {A} (P: A -> A -> Prop) (oa ob: option A): Prop :=
 
 (** This file holds definitions related to our stack abstract data type (ADT).   *)
 
-(** * Stack permissions *)
-
-Inductive stack_permission: Type :=
-  Public
-| Private.
-
-Definition stack_perm_eq: forall (p1 p2: stack_permission), {p1 = p2} + {p1 <> p2}.
-Proof.
-  decide equality.
-Qed.
-
-(** Order on permissions: [Public] is greater than [Private]. Moreover,
-    [stack_perm_le] is reflexive. *)
-
-Definition stack_perm_le (sp1 sp2: stack_permission) :=
-  match sp1, sp2 with
-  | Private, _ => True
-  | Public, Public => True
-  | Public, _ => False
-  end.
-
-Lemma stack_perm_le_refl:
-  forall p,
-    stack_perm_le p p.
-Proof.
-  destruct p; red; auto.
-Qed.
-
-Lemma stack_perm_le_trans:
-  forall p1 p2 p3,
-    stack_perm_le p1 p2 ->
-    stack_perm_le p2 p3 ->
-    stack_perm_le p1 p3.
-Proof.
-  destruct p1,p2,p3; unfold stack_perm_le; intros; congruence.
-Qed.
-
-
 (** * Block information  *)
 
 (** A block information records its size ([frame_size]) and the stack
@@ -71,54 +33,18 @@ Qed.
 Record frame_info :=
   {
     frame_size: Z;
-    frame_perm: Z -> stack_permission;
     frame_size_pos: (0 <= frame_size)%Z;
   }.
 
 Definition public_frame_info sz : frame_info :=
   {|
     frame_size := Z.max 0 sz;
-    frame_perm := fun _ => Public;
     frame_size_pos := Z.le_max_l _ _;
   |}.
-
-Program Definition frame_info_of_size_and_pubrange (size: Z) (pubrange: Z * Z) : option frame_info :=
-  if zlt 0 size
-  then
-    let '(lo,hi) := pubrange in
-    Some {| frame_size := size; frame_perm := fun o => if zle lo o && zlt o hi then Public else Private; |}
-  else None.
-Next Obligation.
-  omega.
-Qed.
-
-Definition frame_public f o := frame_perm f o = Public.
-
-Definition frame_private f o := frame_perm f o = Private.
-
-Definition frame_public_dec: forall f o, {frame_public f o} + {~ frame_public f o}.
-Proof.
-  unfold frame_public; intros; apply stack_perm_eq.
-Qed.
-
-Definition frame_private_dec: forall f o, {frame_private f o} + {~ frame_private f o}.
-Proof.
-  unfold frame_private; intros; apply stack_perm_eq.
-Qed.
-
-Definition public_stack_range (lo hi: Z) (fi: frame_info) : Prop :=
-  forall ofs, (lo <= ofs < hi)%Z -> frame_public fi ofs.
-
-Lemma public_stack_range_lo_ge_hi:
-  forall lo hi fi, (hi <= lo)%Z -> public_stack_range lo hi fi.
-Proof.
-  red; intros; omega.
-Qed.
 
 Program Definition empty_frame: frame_info :=
   {|
     frame_size := 0;
-    frame_perm o := Public;
   |}.
 
 (** * Frame ADT  *)
@@ -140,15 +66,6 @@ Record frame_adt : Type :=
     frame_adt_size_pos:
       (0 <= frame_adt_size)%Z;
   }.
-
-Lemma stack_perm_le_public:
-  forall fi p o,
-    (forall x, frame_perm fi x = Public) ->
-    stack_perm_le p (frame_perm fi o).
-Proof.
-  intros fi p o PUB; rewrite PUB.
-  destruct p; red; auto.
-Qed.
 
 (** * Tailcall frames *)
 
@@ -187,31 +104,33 @@ Definition get_stack_blocks (s: stack) : list block :=
 Definition in_frame (f: frame_adt) (b: block) : Prop :=
   In b (get_frame_blocks f).
 
+(* In top tailcall stage of tailcall frame *)
 Definition in_frames (l: tframe_adt) (b: block) :=
   In b (get_opt_frame_blocks (fst l)).
 
+(* In some top tailcall stage of some taillcall frame in stack *)
 Definition in_stack (s: stack) (b: block) :=
   In b (get_stack_blocks s).
 
 Definition in_frame' (f: frame_adt) bfi :=
   In bfi (frame_adt_blocks f).
 
-Definition in_frames' (tf: tframe_adt) b :=
+Definition in_frames' (tf: tframe_adt) bfi :=
   match fst tf with
-  | Some f => in_frame' f b
+  | Some f => in_frame' f bfi
   | None => False
   end.
 
-Fixpoint in_stack' (s: stack) b :=
+Fixpoint in_stack' (s: stack) bfi :=
   match s with
   | nil => False
-  | tf::s => in_frames' tf b \/ in_stack' s b
+  | tf::s => in_frames' tf bfi \/ in_stack' s bfi
   end.
 
 Lemma in_frames'_rew:
-  forall tf b,
-    in_frames' tf b <->
-    exists fr, in_frame' fr b /\ fst tf = Some fr.
+  forall tf bfi,
+    in_frames' tf bfi <->
+    exists fr, in_frame' fr bfi /\ fst tf = Some fr.
 Proof.
   unfold in_frames'. intros.
   destr; split; intros A; try decompose [ex and] A; try (intuition congruence);
@@ -219,10 +138,10 @@ Proof.
 Qed.
 
 Lemma in_stack'_rew:
-  forall s b,
-    in_stack' s b <->
+  forall s bfi,
+    in_stack' s bfi <->
     exists (tf: tframe_adt),
-      in_frames' tf b /\ In tf s.
+      in_frames' tf bfi /\ In tf s.
 Proof.
   induction s; simpl; split; intros; eauto.
   - easy.
@@ -287,16 +206,6 @@ Proof.
   rewrite map_app, concat_app, in_app; tauto.
 Qed.
 
-(* Lemma in_frames_app: *)
-(*   forall l1 l2 b, *)
-(*     in_frames l1 b \/ in_frames l2 b <-> *)
-(*     in_frames (l1 ++ l2) b. *)
-(* Proof. *)
-(*   intros. *)
-(*   unfold in_frames, get_frames_blocks in *. *)
-(*   rewrite map_app, concat_app, in_app; tauto. *)
-(* Qed. *)
-
 Lemma in_frame_info:
   forall b (f: frame_adt),
     in_frame f b ->
@@ -342,20 +251,13 @@ Definition get_frame_info s : block -> option frame_info :=
 
 (** * Injection of frame information  *)
 
-Record inject_frame_info delta fi fi' :=
-  {
-    inject_perm: forall o, (0 <= o < frame_size fi)%Z -> stack_perm_le (frame_perm fi o) (frame_perm fi' (o + delta));
-    inject_size:
-      forall o, (0 <= o < frame_size fi -> 0 <= o + delta < frame_size fi')%Z;
-  }.
+Definition inject_frame_info delta fi fi' := forall o, (0 <= o < frame_size fi -> 0 <= o + delta < frame_size fi')%Z.
 
 Lemma inject_frame_info_id:
   forall f,
     inject_frame_info 0 f f.
 Proof.
-  constructor; auto.
-  intros; rewrite Z.add_0_r. eapply stack_perm_le_refl; auto.
-  intros; omega.
+  constructor; intros; omega.
 Qed.
 
 Hint Resolve inject_frame_info_id.
@@ -366,43 +268,11 @@ Lemma inject_frame_info_trans:
     inject_frame_info delta2 f2 f3 ->
     inject_frame_info (delta1 + delta2) f1 f3.
 Proof.
-  intros f1 f2 f3 delta1 delta2 A B; inv A; inv B; constructor; eauto.
-  - intros.
-    eapply stack_perm_le_trans; eauto.
-    rewrite Z.add_assoc. eauto.
-  - intros.
-    apply inject_size0 in H. apply inject_size1 in H. omega.
+  intros f1 f2 f3 delta1 delta2 A B; unfold inject_frame_info in A, B; constructor; apply A in H; apply B in H;
+    rewrite Z.add_assoc; destruct H; eauto.
 Qed.
 
 Hint Resolve inject_frame_info_trans.
-
-Lemma public_stack_shift:
-  forall f1 f2 delta,
-    inject_frame_info delta f1 f2 ->
-    forall o,
-      (0 <= o < frame_size f1)%Z ->
-      frame_public f1 o ->
-      frame_public f2 (o+delta).
-Proof.
-  unfold frame_public. intros.
-  generalize (inject_perm _ _ _ H _ H0); eauto.
-  rewrite H1.
-  destruct (frame_perm f2); simpl; intuition.
-Qed.
-
-Lemma public_stack_range_shift:
-  forall f1 f2 delta,
-    inject_frame_info delta f1 f2 ->
-    forall lo hi,
-      (0 <= lo)%Z -> (hi <= frame_size f1)%Z ->
-      public_stack_range lo hi f1 ->
-      public_stack_range (lo+delta) (hi+delta) f2.
-Proof.
-  unfold public_stack_range; intros.
-  replace ofs with (ofs-delta+delta)%Z by omega.
-  eapply public_stack_shift; eauto. omega.
-  apply H2; omega.
-Qed.
 
 (** * Injection of frame_adt  *)
 
@@ -752,23 +622,12 @@ Proof.
   rewrite in_stack_cons; left. eauto.
 Qed.
 
-(** * Surjectivity of stack injections  *)
-
-(* Definition frameinj_surjective (g: frameinj) n2 := *)
-(*   sum_list g = n2. *)
-
-Class InjectPerm :=
-  {
-    inject_perm_condition: permission -> Prop;
-    inject_perm_condition_writable: forall p, perm_order Writable p -> inject_perm_condition p;
-  }.
-
 (** * Specifying tailcalled frames.  *)
 (** A tframe is a non-empty list of frames (a::l). It must be the case that all
     blocks in l have no permission.
  *)
 
-Definition wf_tframe (m: perm_type) (* (j: meminj) *) (tf: tframe_adt) : Prop :=
+Definition wf_tframe (m: perm_type) (tf: tframe_adt) : Prop :=
   forall b,
     forall f,
       In f (snd tf) ->
@@ -780,13 +639,11 @@ Definition wf_stack (m: perm_type) (s: stack) : Prop :=
   Forall (wf_tframe m) s.
 
 Section INJ.
-  Context {injperm: InjectPerm}.
-
    Definition has_perm (m: perm_type) (j: meminj) (f: tframe_adt) : Prop :=
-     exists b o k p, j b <> None /\ in_frames f b /\ m b o k p /\ inject_perm_condition p.
+     exists b o k p, j b <> None /\ in_frames f b /\ m b o k p.
 
    Definition has_perm_frame (m: perm_type) (j: meminj) (f: frame_adt) : Prop :=
-     exists b o k p, j b <> None /\ in_frame f b /\ m b o k p /\ inject_perm_condition p.
+     exists b o k p, j b <> None /\ in_frame f b /\ m b o k p.
 
    Definition tframe_inject (f: meminj) (P: perm_type) (tf1 tf2: tframe_adt): Prop :=
      forall f1,
@@ -806,7 +663,7 @@ Section INJ.
    Lemma tframe_inject_id P a:
      tframe_inject inject_id P a a.
    Proof.
-     apply self_tframe_inject. right; reflexivity.
+     apply self_tframe_inject. right. reflexivity.
    Qed.
 
    Lemma tframe_inject_incr:
@@ -819,7 +676,7 @@ Section INJ.
        tframe_inject f P f1 f2 ->
        tframe_inject f' P f1 f2.
    Proof.
-     intros P f f' f1 f2 INCR NEW TF ff1 IN1 (b & o & k & p & Fnone & IFR & PERM & IPC).
+     intros P f f' f1 f2 INCR NEW TF ff1 IN1 (b & o & k & p & Fnone & IFR & PERM).
      edestruct TF as (f0 & IN & FI); eauto.
      - red.
        repeat eexists; eauto.
@@ -840,12 +697,11 @@ Section INJ.
        (PERMS: forall b1 b2 delta o k p,
            f b1 = Some (b2, delta) ->
            P b1 o k p ->
-           inject_perm_condition p ->
            P' b2 (o + delta)%Z k p),
        tframe_inject (compose_meminj f f') P l1 l3.
    Proof.
      intros f f' P P' l1 l2 FI12 l3 FI23 PERMS
-            f1 INf1 (b & o & k & p & JB & IFR & PERM & IPC).
+            f1 INf1 (b & o & k & p & JB & IFR & PERM).
      unfold compose_meminj in JB; repeat destr_in JB. subst.
      edestruct FI12 as (f2 & INl2 & FI12'); eauto.
      repeat eexists; eauto. congruence.
@@ -856,51 +712,51 @@ Section INJ.
      eapply frame_inject_compose; eauto.
    Qed.
 
-   Inductive stack_inject_aux (f: meminj) (m: perm_type) : frameinj -> stack -> stack -> Prop :=
-   | stack_inject_aux_intro:
-       stack_inject_aux f m nil nil nil
-   | stack_inject_aux_cons
+   Inductive stack_inject (f: meminj) (m: perm_type) : frameinj -> stack -> stack -> Prop :=
+   | stack_inject_intro:
+       stack_inject f m nil nil nil
+   | stack_inject_cons
        n g s1 hs1 ts1 tf ts2
        (TAKE: take (S n) s1 = Some hs1)
        (DROP: drop (S n) s1 = ts1)
-       (SIA_REC: stack_inject_aux f m g ts1 ts2)
+       (SIA_REC: stack_inject f m g ts1 ts2)
        (FI: Forall (fun f1 => tframe_inject f m f1 tf) hs1):
-     stack_inject_aux f m (S n::g) s1 (tf::ts2).
+     stack_inject f m (S n::g) s1 (tf::ts2).
 
-   Lemma stack_inject_aux_length_l:
+   Lemma stack_inject_length_l:
      forall f m g s1 s2,
-       stack_inject_aux f m g s1 s2 ->
+       stack_inject f m g s1 s2 ->
        sum_list g = length s1.
    Proof.
      induction 1; simpl; intros; eauto.
      rewrite (take_drop _ _ _ TAKE). subst.
-     rewrite IHstack_inject_aux. rewrite app_length.
+     rewrite IHstack_inject. rewrite app_length.
      f_equal. symmetry.
      erewrite take_length by eauto. omega.
    Qed.
 
-   Lemma stack_inject_aux_length_r:
+   Lemma stack_inject_length_r:
      forall f m g s1 s2,
-       stack_inject_aux f m g s1 s2 ->
+       stack_inject f m g s1 s2 ->
        length g = length s2.
    Proof.
      induction 1; simpl; intros; eauto.
    Qed.
 
-   Record stack_inject (f: meminj) (g: frameinj) (m: perm_type) (s1 s2: stack) :=
-    {
-      (* stack_src_wf: wf_stack m s1; *)
-      stack_inject_frame_inject: stack_inject_aux f m g s1 s2;
-      stack_inject_not_in_source:
-        forall b1 b2 delta bi2
-          (FB: f b1 = Some (b2, delta))
-          (NIS: ~ in_stack s1 b1)
-          (FI: in_stack' s2 (b2,bi2))
-          o k p
-          (PERM: m b1 o k p)
-          (IPC: inject_perm_condition p),
-          frame_public bi2 (o + delta);
-    }.
+  Close Scope nat_scope.
+
+  Lemma stack_inject_flat:
+    forall s P f (F: forall b, f b = None \/ f b = Some (b, 0)),
+     stack_inject f P (flat_frameinj (length s)) s s.
+  Proof.
+    induction s; simpl; intros.
+    constructor.
+    simpl. econstructor. reflexivity. reflexivity. simpl. eauto.
+    repeat constructor.
+    apply self_tframe_inject; auto.
+  Qed.
+
+  Open Scope nat_scope.
 
   Lemma concat_In:
     forall {A} (l: list (list A)) b,
@@ -943,22 +799,20 @@ Section INJ.
 
   Lemma stack_inject_compat:
     forall f g P s1 s2,
-      stack_inject f g P s1 s2 ->
+      stack_inject f P g s1 s2 ->
     forall b1 b2 delta bi1,
       f b1 = Some (b2, delta) ->
       in_stack' s1 (b1, bi1) ->
-      (exists o k p, P b1 o k p /\ inject_perm_condition p) ->
+      (exists o k p, P b1 o k p) ->
       exists bi2,
         in_stack' s2 (b2, bi2) /\ inject_frame_info delta bi1 bi2.
   Proof.
     intros f g P s1 s2 SI.
-    inv SI.
-    revert stack_inject_frame_inject0 .
-    clear stack_inject_not_in_source0.
+    revert SI.
     induction 1; simpl; intros b1 b2 delta bi1 FB INS PERM.
     - easy.
     - subst.
-      destruct PERM as (o & k & p & PERM & IPC).
+      destruct PERM as (o & k & p & PERM).
       rewrite (take_drop _ _ _ TAKE) in INS.
       rewrite in_stack'_app in INS.
       destruct INS as [INS|INS].
@@ -977,7 +831,7 @@ Section INJ.
         destruct FI as (bi2 & INfr2 & IFI).
         exists bi2; split; auto. left; rewrite in_frames'_rew.
         eexists; split; eauto.
-      + edestruct IHstack_inject_frame_inject0 as (bi2 & INS2 & IFI); eauto.
+      + edestruct IHSI as (bi2 & INS2 & IFI); eauto.
   Qed.
 
   Lemma stack_top_in_frames:
@@ -1004,9 +858,9 @@ Section INJ.
 
   Lemma tframe_inject_in_frames:
     forall f m v1 v2 b b' delta o k p,
-      tframe_inject f m v1 v2 -> m b o k p -> inject_perm_condition p -> in_frames v1 b -> f b = Some (b', delta) -> in_frames v2 b'.
+      tframe_inject f m v1 v2 -> m b o k p -> in_frames v1 b -> f b = Some (b', delta) -> in_frames v2 b'.
   Proof.
-    intros f m v1 v2 b b' delta o k p TFI PERM IPC IFR FB.
+    intros f m v1 v2 b b' delta o k p TFI PERM IFR FB.
     red in IFR. unfold get_opt_frame_blocks in IFR.
     destr_in IFR; try easy. unfold get_frame_blocks in IFR.
     rewrite in_map_iff in IFR. destruct IFR as (fa & blocks & IN). subst.
@@ -1022,22 +876,22 @@ Section INJ.
 
   Lemma stack_inject_is_stack_top:
     forall f g m s1 s2,
-      stack_inject f g m s1 s2 ->
+      stack_inject f m g s1 s2 ->
       forall b1 b2 delta,
         f b1 = Some (b2, delta) ->
-        (exists o k p, m b1 o k p /\ inject_perm_condition p) ->
+        (exists o k p, m b1 o k p) ->
         is_stack_top s1 b1 ->
         is_stack_top s2 b2.
   Proof.
     intros f g m s1 s2 SI b1 b2 delta FB PERM IST.
     destruct (stack_top_frame_at_position _ _ IST) as (ff & FAP1 & IFR1).
     destruct s1. inv FAP1. simpl in *. congruence.
-    inv SI. inv stack_inject_frame_inject0.
+    inv SI.
     eapply frame_at_position_stack_top; eauto.
     constructor. reflexivity.
     inv FAP1. inv H.
     simpl in TAKE. destr_in TAKE. inv TAKE. inv FI.
-    destruct PERM as (o & k & p & PERM & IPC).
+    destruct PERM as (o & k & p & PERM).
     eapply tframe_inject_in_frames; eauto.
   Qed.
 
@@ -1098,37 +952,6 @@ Section INJ.
       exfalso; eapply H6. eauto. eapply in_frames_in_stack; eauto.
       inv H. eapply IHl; eauto.
   Qed.
-
-  (* Inductive nodupt: tframe_adt -> Prop := *)
-  (* | nodupt_nil: nodupt nil *)
-  (* | nodupt_cons: forall f s, nodupt s -> (forall b, in_frame f b -> ~ in_frames s b) -> nodupt (f::s). *)
-
-  (* Definition nodupt (s: tframe_adt) := *)
-  (*   forall b f1 f2, *)
-  (*     In f1 s -> *)
-  (*     In f2 s -> *)
-  (*     in_frame f1 b -> *)
-  (*     in_frame f2 b -> *)
-  (*     f1 = f2. *)
-
-
-  (* Lemma nodupt_nodupt': forall l, nodupt l -> nodupt' l. *)
-  (* Proof. *)
-  (*   induction 1; simpl; intros; eauto. *)
-  (*   - unfold nodupt'. easy. *)
-  (*   - intros b f1 f2 [EQ1|AIN1] [EQ2|AIN2] IFR1 IFR2; subst; simpl in *; auto. *)
-  (*     + eapply H0 in IFR1. elim IFR1. *)
-  (*       unfold in_frames, get_frames_blocks. *)
-  (*       apply concat_In. *)
-  (*       eexists; split. apply IFR2. *)
-  (*       apply in_map. simpl. auto. *)
-  (*     + eapply H0 in IFR2. elim IFR2. *)
-  (*       unfold in_frames, get_frames_blocks. *)
-  (*       apply concat_In. *)
-  (*       eexists; split. apply IFR1. *)
-  (*       apply in_map. simpl. auto. *)
-  (*     + eapply IHnodupt; eauto. *)
-  (* Qed. *)
 
   Lemma in_frames_in_frame_ex:
     forall tf b,
@@ -1323,7 +1146,7 @@ Section INJ.
 
   Lemma stack_inject_inject_frame_info:
     forall f g m l1 l2,
-      stack_inject f g m l1 l2 ->
+      stack_inject f m g l1 l2 ->
       nodup l1 ->
       nodup l2 ->
       forall b1 bi1 b2 bi2,
@@ -1333,12 +1156,11 @@ Section INJ.
           f b1 = Some (b2, delta) ->
           forall o k p,
             m b1 o k p ->
-            inject_perm_condition p ->
         inject_frame_info delta bi1 bi2.
   Proof.
     intros f g m l1 l2 SI ND1 ND2 b1 bi1 b2 bi2 INS1 INS2 delta FB o k p PERM IPC.
     edestruct (stack_inject_compat _ _ _ _ _ SI _ _ _ _ FB INS1) as (bi2' & INS2' & IFI).
-    do 3 eexists; split; eauto.
+    do 3 eexists; eauto.
     cut (bi2 = bi2'). intro; subst; auto.
     eapply in_stack'_norepet; eauto.
   Qed.
@@ -1366,14 +1188,14 @@ Section INJ.
       drop n1 (drop n2 l) = drop (n1 + n2) l.
   Proof.
     induction n1; simpl; intros; eauto.
-    rewrite <- IHn1. rewrite drop_tl. auto.
+    rewrite <- IHn1. rewrite drop_tl. reflexivity.
   Qed.
 
   Lemma stack_inject_drop:
     forall f m1 g1 l1 l2
-      (SI : stack_inject_aux f m1 g1 l1 l2)
+      (SI : stack_inject f m1 g1 l1 l2)
       n (POS: O < n) l (TAKE : take n g1 = Some l),
-      stack_inject_aux f m1 (drop n g1) (drop (sum_list l) l1) (drop n l2).
+      stack_inject f m1 (drop n g1) (drop (sum_list l) l1) (drop n l2).
   Proof.
     induction 1; simpl; intros; eauto.
     - destruct n; simpl in *; inv TAKE. simpl. constructor.
@@ -1405,15 +1227,15 @@ Section INJ.
     repeat destr_in H. simpl. eauto.
   Qed.
 
-  Lemma stack_inject_aux_take:
+  Lemma stack_inject_take:
     forall n
       f m g s1 s2
-      (SIA: stack_inject_aux f m g s1 s2)
+      (SIA: stack_inject f m g s1 s2)
       g' s1' s2'
       (TG: take n g = Some g')
       (TS1: take (sum_list g') s1 = Some s1')
       (TS2: take n s2 = Some s2'),
-      stack_inject_aux f m g' s1' s2'.
+      stack_inject f m g' s1' s2'.
   Proof.
     induction n; simpl; intros.
     - inv TG; inv TS2. simpl in *. inv TS1. constructor.
@@ -1424,9 +1246,9 @@ Section INJ.
       eapply take_drop_rest; eauto.
   Qed.
 
-  Lemma stack_inject_aux_tframe_inject:
+  Lemma stack_inject_tframe_inject:
     forall f m g s1 s2 x,
-      stack_inject_aux f m g s1 s2 ->
+      stack_inject f m g s1 s2 ->
       In x s1 ->
       exists y, In y s2 /\ tframe_inject f m x y.
   Proof.
@@ -1435,23 +1257,22 @@ Section INJ.
     rewrite (take_drop _ _ _ TAKE) in H0. rewrite in_app in H0.
     destruct H0.
     rewrite Forall_forall in FI. apply FI in H0. eauto.
-    destruct IHstack_inject_aux as (y & INs2 & TFI). auto.
+    destruct IHstack_inject as (y & INs2 & TFI). auto.
     eauto.
   Qed.
 
   Opaque take drop.
 
-  Lemma stack_inject_aux_compose:
+  Lemma stack_inject_compose_aux:
     forall f f' m1 m2 g1 g2 s1 s2 s3 g3
       (COMP : compose_frameinj g1 g2 = Some g3)
-      (SI12 : stack_inject_aux f m1 g1 s1 s2)
-      (SI23 : stack_inject_aux f' m2 g2 s2 s3)
+      (SI12 : stack_inject f m1 g1 s1 s2)
+      (SI23 : stack_inject f' m2 g2 s2 s3)
       (PERMS: forall b1 b2 delta o k p,
           f b1 = Some (b2, delta) ->
           m1 b1 o k p ->
-          inject_perm_condition p ->
           m2 b2 (o + delta)%Z k p),
-      stack_inject_aux (compose_meminj f f') m1 g3 s1 s3.
+      stack_inject (compose_meminj f f') m1 g3 s1 s3.
   Proof.
     intros.
     revert f' m2 g2 s2 s3 SI23 f m1 g1 s1 SI12 g3 COMP PERMS.
@@ -1460,7 +1281,7 @@ Section INJ.
     - repeat destr_in COMP.
       repeat destr_in H0. repeat destr_in Heqo. simpl in *.
       destruct (take_succeeds (sum_list l) s0) as (t & EQ).
-      erewrite <- stack_inject_aux_length_l by eauto.
+      erewrite <- stack_inject_length_l by eauto.
       eapply take_sumlist; eauto.
       cut (exists sl, sum_list l = S sl). intros (sl & SL). rewrite SL in *.
       econstructor; eauto.
@@ -1468,9 +1289,9 @@ Section INJ.
       rewrite <- SL.
       eapply stack_inject_drop; eauto. omega.
       rewrite Forall_forall in FI |- *. intros.
-      exploit stack_inject_aux_take. apply SI12. eauto. rewrite SL; eauto. eauto. 
+      exploit stack_inject_take. apply SI12. eauto. rewrite SL; eauto. eauto. 
       intro SIA.
-      edestruct (stack_inject_aux_tframe_inject _ _ _ _ _ x SIA) as (y & INhs1 & TFI). auto.
+      edestruct (stack_inject_tframe_inject _ _ _ _ _ x SIA) as (y & INhs1 & TFI). auto.
       eapply tframe_inject_compose; eauto.
       Transparent take drop.
       inv SI12; simpl in *. congruence.
@@ -1479,97 +1300,38 @@ Section INJ.
 
   Lemma stack_inject_compose:
     forall (f f' : meminj) g g' m1 l1 l2,
-      stack_inject f g m1 l1 l2 ->
+      stack_inject f m1 g l1 l2 ->
       forall m2 l3,
-        stack_inject f' g' m2 l2 l3 ->
+        stack_inject f' m2 g' l2 l3 ->
         nodup l2 ->
         nodup l3 ->
         (forall b1 b2 delta o k p,
             f b1 = Some (b2, delta) ->
             m1 b1 o k p ->
-            inject_perm_condition p ->
             m2 b2 (o + delta)%Z k p) ->
         stack_agree_perms m2 l2 ->
         forall g3,
         (compose_frameinj g g') = Some g3 ->
-        stack_inject (compose_meminj f f') g3 m1 l1 l3.
+        stack_inject (compose_meminj f f') m1 g3 l1 l3.
   Proof.
     intros f f' g g' m1 l1 l2 SI1 m2 l3 SI2 ND2 ND3 PERM FAP g3 COMP.
-    inversion SI1; inversion SI2.
-    split; auto.
-    - eapply stack_inject_aux_compose; eauto.
-    - intros b1 b3 delta bi3 CINJ NIS1 INS3 o k p PERMS IPC.
-      unfold compose_meminj in CINJ.
-      destruct (f b1) as [[b2 delta1]|] eqn:FB1; try congruence.
-      destruct (f' b2) as [[b33 delta2]|] eqn:FB2; try congruence.
-      inv CINJ.
-      destruct (in_stack_dec l2 b2).
-      +
-        assert (INS2: exists bi2, in_stack' l2 (b2,bi2)).
-        {
-          destruct (in_stack_in_frames_ex _ _ i) as (f2 & INS2 & INF2).
-          setoid_rewrite in_stack'_rew.
-          edestruct in_frames_in_frame_ex as (f2' & INS2' & INF2'). apply INF2.
-          edestruct in_frame_info as (bi2 & IFR2). apply INF2'.
-          setoid_rewrite in_frames'_rew.
-          exists bi2, f2. split; auto.
-          exists f2'; split; auto.
-        }
-        destruct INS2 as (bi2 & INS2).
-        exploit stack_inject_not_in_source0. eauto. eauto. eauto. eauto. auto.
-        intro PUB2.
-        exploit PERM; eauto. intro PERMS2.
-        rewrite Z.add_assoc. eapply public_stack_shift; eauto.
-        2: eapply in_stack'_stack_agree_perms; eauto.
-        eapply stack_inject_inject_frame_info; eauto.
-      + rewrite Z.add_assoc. eapply stack_inject_not_in_source1; eauto.
+    eapply stack_inject_compose_aux; eauto.
   Qed.
 
-  Definition public_stack_access l (b: block) (lo hi: Z) : Prop :=
-    match get_frame_info l b with
-      Some fi => public_stack_range lo hi fi
-    | None => True
-    end.
-
-  Lemma lo_ge_hi_public_stack_access:
-    forall m b lo hi,
-      (lo >= hi)%Z ->
-      public_stack_access m b lo hi.
-  Proof.
-    red. intros.
-    destruct (get_frame_info m b); try tauto.
-    red; intros. omega.
-  Qed.
-
-  Definition stack_access (m: stack) (b: block) (lo hi: Z) : Prop :=
-    is_stack_top m b \/ public_stack_access m b lo hi.
-
-  Lemma is_stack_top_dec : forall m b,
-      {is_stack_top m b} + {~is_stack_top m b}.
+  Lemma is_stack_top_dec : forall s b,
+      {is_stack_top s b} + {~is_stack_top s b}.
   Proof.
     intros. unfold is_stack_top. apply in_dec. 
     apply eq_block.
   Qed.
 
-  Lemma lo_ge_hi_stack_access:
-    forall m b lo hi,
-      (lo >= hi)%Z ->
-      stack_access m b lo hi.
-  Proof.
-    unfold stack_access.
-    intros.
-    destruct (is_stack_top_dec m b);[left|right]. auto.
-    eapply lo_ge_hi_public_stack_access. auto.
-  Qed.
-
-
   Lemma is_stack_top_stack_blocks:
-    forall m b,
-      is_stack_top m b <-> (exists f r, in_frames f b /\ m = f::r).
+    forall s b,
+      is_stack_top s b <-> (exists f r, in_frames f b /\ s = f::r).
   Proof.
     unfold is_stack_top, get_stack_top_blocks.
     intros.
-    destruct m eqn:?; intuition.
+    destruct s eqn:?; intuition.
     - decompose [ex and] H; intuition congruence.
     - repeat eexists. eauto.
     - subst.    
@@ -1577,82 +1339,13 @@ Section INJ.
       eauto. 
   Qed.
 
-  Lemma in_stack_data_inside:
-    forall fi lo hi lo' hi',
-      public_stack_range lo hi fi ->
-      (lo <= lo')%Z ->
-      (hi' <= hi)%Z ->
-      public_stack_range lo' hi' fi.
-  Proof.
-    intros fi lo hi lo' hi' NPSA LO HI.
-    do 2 red in NPSA |- *.
-    intros; apply NPSA. omega.
-  Qed.
-
-  Lemma public_stack_access_inside:
-    forall m b lo hi lo' hi',
-      public_stack_access m b lo hi ->
-      (lo <= lo')%Z ->
-      (hi' <= hi)%Z ->
-      public_stack_access m b lo' hi'.
-  Proof.
-    intros m b lo hi lo' hi' NPSA LO HI.
-    unfold public_stack_access in *.
-    destruct (get_frame_info m b); auto.
-    eapply in_stack_data_inside in NPSA; eauto.
-  Qed.
-
-  Lemma stack_access_inside:
-    forall m b lo hi lo' hi',
-      stack_access m b lo hi ->
-      (lo <= lo')%Z ->
-      (hi' <= hi)%Z ->
-      stack_access m b lo' hi'.
-  Proof.
-    intros m b lo hi lo' hi' NPSA LO HI.
-    unfold stack_access in *.
-    destruct NPSA; auto. right.
-    eapply public_stack_access_inside; eauto.
-  Qed.
-
-  Lemma public_stack_range_dec : forall lo hi f,
-      {public_stack_range lo hi f} + {~public_stack_range lo hi f}.
-  Proof.
-    unfold public_stack_range. intros. 
-    edestruct (Intv.forall_rec (frame_public f) (fun ofs => ~ frame_public f ofs)) with (lo:=lo) (hi:=hi).
-    - apply frame_public_dec. 
-    - auto.
-    - right. intro A.
-      destruct e as (x & IN & NIN).
-      apply NIN. apply A. auto.
-  Qed.
-
-  Lemma public_stack_access_dec : forall m b lo hi,
-      {public_stack_access m b lo hi} + 
-      {~public_stack_access m b lo hi}.
-  Proof.
-    unfold public_stack_access.
-    intros.
-    destruct (get_frame_info m b); auto.
-    apply public_stack_range_dec.
-  Qed.
-
-  Lemma stack_access_dec : forall m b lo hi,
-      {stack_access m b lo hi} + 
-      {~stack_access m b lo hi}.
-  Proof.
-    intros. unfold stack_access.
-    destruct (is_stack_top_dec m b); auto.
-    destruct (public_stack_access_dec m b lo hi); auto.
-    right; intuition.
-  Qed.
-
-
   Lemma not_in_frames_no_frame_info:
-    forall (m : tframe_adt) (b : block), ~ in_frames m b -> get_assoc_tframes m b = None.
+    forall (tf : tframe_adt) (b : block), 
+      ~ in_frames tf b -> 
+      get_assoc_tframes tf b = None.
   Proof.
     intros.
-    destruct (get_assoc_tframes m b) eqn:GAT; auto.
+    destruct (get_assoc_tframes tf b) eqn:GAT; auto.
     apply get_assoc_tframes_in in GAT.
     destruct GAT as (f0 & IN1 & IN2).
     exfalso; apply H.
@@ -1661,25 +1354,25 @@ Section INJ.
   Qed.
 
   Lemma get_frame_info_in_frames:
-    forall m b f, get_assoc_tframes m b = Some f -> in_frames m b.
+    forall tf b f, get_assoc_tframes tf b = Some f -> in_frames tf b.
   Proof.
     intros.
-    destruct (in_frames_dec m b); auto.
+    destruct (in_frames_dec tf b); auto.
     rewrite not_in_frames_no_frame_info in H; auto. congruence.
   Qed.
 
   Lemma get_frame_info_in_stack:
-    forall m b f, get_frame_info m b = Some f -> in_stack m b.
+    forall s b f, get_frame_info s b = Some f -> in_stack s b.
   Proof.
     intros.
-    destruct (in_stack_dec m b); auto.
+    destruct (in_stack_dec s b); auto.
     rewrite not_in_stack_get_assoc in H; auto. congruence.
   Qed.
 
-  Inductive option_le_stack {A: Type} (Pns: A -> Prop) (Pss: A -> A -> Prop) (delta: Z): option A -> option A -> Prop :=
-  | option_le_none_none : option_le_stack Pns Pss delta None None
-  | option_le_some_some a b : Pss a b -> option_le_stack Pns Pss delta (Some a) (Some b)
-  | option_le_none_some a: Pns a -> option_le_stack Pns Pss delta None (Some a).
+  Inductive option_le_stack {A: Type} (Pns: A -> Prop) (Pss: A -> A -> Prop): option A -> option A -> Prop :=
+  | option_le_none_none : option_le_stack Pns Pss None None
+  | option_le_some_some a b : Pss a b -> option_le_stack Pns Pss (Some a) (Some b)
+  | option_le_none_some a: Pns a -> option_le_stack Pns Pss None (Some a).
 
   Lemma get_assoc_spec:
     forall s b fi,
@@ -1708,7 +1401,7 @@ Section INJ.
   Lemma in_frame_get_assoc:
     forall a b,
       in_frame a b ->
-      exists f : frame_info, get_assoc positive frame_info peq (frame_adt_blocks a) b = Some f.
+      exists fi : frame_info, get_assoc positive frame_info peq (frame_adt_blocks a) b = Some fi.
   Proof.
     unfold in_frame, get_frame_blocks.
     intros a.
@@ -1721,7 +1414,7 @@ Section INJ.
   Lemma in_frames_get_assoc_tframes:
     forall s b,
       in_frames s b ->
-      exists f, get_assoc_tframes s b = Some f.
+      exists fi, get_assoc_tframes s b = Some fi.
   Proof.
     unfold in_frames, get_assoc_tframes. intros. destr; try easy.
     rewrite pred_dec_true.
@@ -1731,7 +1424,7 @@ Section INJ.
   Lemma in_stack_get_assoc_stack:
     forall s b,
       in_stack s b ->
-      exists f, get_assoc_stack s b = Some f.
+      exists fi, get_assoc_stack s b = Some fi.
   Proof.
     induction s; simpl; intros; eauto. easy.
     rewrite in_stack_cons in H.
@@ -1742,18 +1435,13 @@ Section INJ.
 
   Lemma get_frame_info_inj_gen:
     forall f g m1 s1 s2 b1 b2 delta
-      (SI: stack_inject f g m1 s1 s2)
+      (SI: stack_inject f m1 g s1 s2)
       (ND1: nodup s1)
       (ND2: nodup s2)
       (FB : f b1 = Some (b2, delta))
-      (PERM: exists o k p, m1 b1 o k p /\ inject_perm_condition p),
-      option_le_stack (fun fi => 
-                   forall ofs k p,
-                     m1 b1 ofs k p ->
-                     inject_perm_condition p ->
-                     frame_public fi (ofs + delta))
+      (PERM: exists o k p, m1 b1 o k p),
+      option_le_stack (fun fi => True)
                 (inject_frame_info delta)
-                delta
                 (get_frame_info s1 b1)
                 (get_frame_info s2 b2).
   Proof.
@@ -1762,7 +1450,7 @@ Section INJ.
     destruct (in_stack_dec s1 b1).
     edestruct in_stack_in_frames_ex as (ff & INS & INF); eauto.
     destruct (get_assoc_stack s1 b1) eqn:STK1.
-    - destruct PERM as (o & k & p & PERM & IPC).
+    - destruct PERM as (o & k & p & PERM).
       eapply (wf_stack_in_frames_in_frame) in INF; eauto.
       destruct INF as (vf1 & VF1 & INF).
       edestruct in_frame_info as (fi2 & INF2); eauto.
@@ -1781,77 +1469,19 @@ Section INJ.
       destruct (get_assoc_stack s2 b2) eqn:FI2.
       + apply option_le_none_some.
         edestruct get_assoc_spec as (fr & tfr & IN & AIN & INR); eauto.
-        intros; eapply stack_inject_not_in_source; eauto.
-        rewrite in_stack'_rew. setoid_rewrite in_frames'_rew.
-        exists tfr. split. exists fr; split; auto. auto.
       + apply option_le_none_none.
   Qed.
 
   Lemma is_stack_top_inj_gen:
     forall P f g s1 s2 b1 b2 delta
-      (MINJ: stack_inject f g P s1 s2)
+      (MINJ: stack_inject f P g s1 s2)
       (FB: f b1 = Some (b2, delta))
-      (PERM: exists o k p, P b1 o k p /\ inject_perm_condition p)
+      (PERM: exists o k p, P b1 o k p)
       (IST: is_stack_top s1 b1),
       is_stack_top s2 b2.
   Proof.
     intros.
     eapply stack_inject_is_stack_top; eauto.
-  Qed.
-
-  Lemma stack_access_inj_gen:
-    forall f g m1 s1 s2 b1 b2 delta lo hi p
-      (MINJ : stack_inject f g m1 s1 s2)
-      (ND1: nodup s1)
-      (ND2: nodup s2)
-      (FAP: stack_agree_perms m1 s1)
-      (FB : f b1 = Some (b2, delta))
-      (RP: forall o, (lo <= o < hi)%Z -> m1 b1 o Cur p)
-      (IPC: inject_perm_condition p)
-      (NPSA: stack_access s1 b1 lo hi),
-      stack_access s2 b2 (lo + delta) (hi + delta).
-  Proof.
-    unfold stack_access, public_stack_access.
-    intros. revert NPSA.
-    destruct (zlt lo hi).
-    intros [A|A].
-    - exploit is_stack_top_inj_gen; eauto.
-      exists lo, Cur, p; split; eauto. apply RP. omega.
-    - assert (forall fi, get_frame_info s2 b2 = Some fi -> public_stack_range (lo+delta) (hi+delta) fi).
-      {
-        intros.
-        assert (in_stack s2 b2).
-        exploit get_assoc_spec. eauto. intros (fr & tf & IN1 & AIN & IN2).
-        eapply in_frames_in_stack; eauto.
-        eapply in_frame_in_frames; eauto.
-        eapply in_frame_blocks_in_frame; eauto.
-        generalize (get_frame_info_inj_gen _ _ _ _ _ _ _ _ MINJ ND1 ND2 FB). rewrite H. intro GFIJ.
-        trim GFIJ.
-        {
-          exists lo, Cur, p; split; eauto. apply RP; omega.
-        }
-        inv GFIJ.
-        - rewrite <- H1 in A.
-          symmetry in H1. apply get_assoc_spec in H1.
-          destruct H1 as (fr & tf & IN1 & AIN & IN2).
-          specialize (FAP _ IN2 _ AIN).
-          red in FAP.
-          assert (forall o, lo <= o < hi -> 0 <= o < frame_size a)%Z as INFR.
-          intros.
-          eapply FAP. eauto. apply RP. auto.
-          destruct (zlt lo hi).
-          + eapply public_stack_range_shift; eauto.
-            apply INFR; auto. omega.
-            cut (hi - 1 < frame_size a)%Z. omega.
-            apply INFR; auto. omega.
-          + eapply public_stack_range_lo_ge_hi. omega.
-        - red.  intros.
-          replace ofs with (ofs-delta+delta)%Z by omega. eapply H3.
-          apply RP. omega. auto.
-      }     
-      right; destr.
-      specialize (H _ eq_refl). auto.
-    - intros; destr. right. eapply public_stack_range_lo_ge_hi. omega.
   Qed.
 
 Lemma in_stack_tl:
@@ -1862,16 +1492,6 @@ Proof.
   destruct l; simpl; auto.
   intros; rewrite in_stack_cons; auto.
 Qed.
-
-
-(* Lemma in_frames_tl: *)
-(*   forall l b, *)
-(*     in_frames ((tl l)) b -> *)
-(*     in_frames (l) b. *)
-(* Proof. *)
-(*   destruct l; simpl; auto. *)
-(*   intros; rewrite in_frames_cons; auto. *)
-(* Qed. *)
 
 Lemma Forall_tl:
   forall {A} P (l: list A),
@@ -1910,7 +1530,7 @@ Lemma tframe_inject_invariant:
 Proof.
   intros m m' f f1 f2 thr PERMS PLT TFI ff1 INf1 HP.
   specialize (TFI _ INf1).
-  trim TFI. destruct HP as (b & o & k & p & FB & IFR & PERM & IPC).
+  trim TFI. destruct HP as (b & o & k & p & FB & IFR & PERM).
   destruct (f b) eqn:?; try congruence. destruct p0.
   repeat eexists; eauto. congruence. eapply PERMS; eauto.
   eapply PLT; eauto. eapply in_frame_in_frames; eauto.
@@ -1927,7 +1547,7 @@ Lemma tframe_inject_invariant_strong:
     tframe_inject f m' f1 f2.
 Proof.
   intros m m' f f1 f2 PERMS TFI ff1 INf1 HP.
-  specialize (TFI _ INf1). trim TFI. destruct HP as (b & o & k & p & FB & IFR & PERM & IPC).
+  specialize (TFI _ INf1). trim TFI. destruct HP as (b & o & k & p & FB & IFR & PERM).
   destruct (f b) eqn:?; try congruence. destruct p0.
   repeat eexists; eauto. congruence.
   destruct TFI as (f3 & EQ & FI).
@@ -1946,9 +1566,11 @@ Proof.
 Qed.
 
 
+(* Either in top of taillcall stage or in past stages *)
 Definition in_frames_all (tf: tframe_adt) b : Prop :=
   In b (get_opt_frame_blocks (fst tf)) \/ exists f, In f (snd tf) /\ in_frame f b.
 
+(* In either the top or past stages of some taillframe *)
 Fixpoint in_stack_all (s: stack) b : Prop :=
   match s with
     nil => False
@@ -1956,11 +1578,11 @@ Fixpoint in_stack_all (s: stack) b : Prop :=
   end.
 
 Lemma in_frames_in_frames_all:
-  forall s b,
-    in_frames s b ->
-    in_frames_all s b.
+  forall tf b,
+    in_frames tf b ->
+    in_frames_all tf b.
 Proof.
-  induction s; simpl; intros; eauto.
+  induction tf; simpl; intros; eauto.
   rewrite in_frames_cons in H. destruct H as (fa & EQ & IFR). red. subst. simpl. left; auto.
 Qed.
 
@@ -2005,7 +1627,7 @@ Lemma tframe_inject_invariant':
 Proof.
   intros m m' f f1 f2 PERMS TFI ff1 INf1 HP.
   specialize (TFI _ INf1).
-  trim TFI. destruct HP as (b & o & k & p & FB & IFR & PERM & IPC).
+  trim TFI. destruct HP as (b & o & k & p & FB & IFR & PERM).
   destruct (f b) eqn:?; try congruence. destruct p0.
   repeat eexists; eauto. congruence. eapply PERMS; eauto.
   left. rewrite INf1. simpl. auto.
@@ -2015,14 +1637,14 @@ Qed.
 
 Lemma stack_inject_aux_invariant:
   forall (m m': perm_type) f g s1 s2,
-    stack_inject_aux f m g s1 s2 ->
+    stack_inject f m g s1 s2 ->
     (forall b ofs k p,
         in_stack_all s1 b ->
         m' b ofs k p -> m b ofs k p) ->
-    stack_inject_aux f m' g s1 s2.
+    stack_inject f m' g s1 s2.
 Proof.
   induction 1; simpl; intros PERM; econstructor; eauto.
-  - eapply IHstack_inject_aux; eauto. subst.
+  - eapply IHstack_inject; eauto. subst.
     intros; eapply PERM; eauto using in_stack_all_drop.
   - eapply Forall_impl. 2: apply FI.
     simpl.
@@ -2036,52 +1658,21 @@ Lemma stack_inject_invariant:
   forall (m m': perm_type) f g s1 s2,
     (forall b ofs k p,
         in_stack_all s1 b ->
-        m' b ofs k p -> m b ofs k p) ->
-    (forall b1 b2 delta, f b1 = Some (b2, delta) ->
-                    ~ in_stack s1 b1 ->
-                    forall fi,
-                      in_stack' s2 (b2,fi) ->
-                      forall o k pp,
-                        m' b1 o k pp ->
-                        inject_perm_condition pp ->
-                        frame_public fi (o + delta)) ->
-    stack_inject f g m s1 s2 ->
-    stack_inject f g m' s1 s2.
+        m' b ofs k p -> m b ofs k p) -> (* just removed stuff here *)
+    stack_inject f m  g s1 s2 ->
+    stack_inject f m' g s1 s2.
 Proof.
-  intros m m' f g s1 s2 PERM PLT FI.
-  destruct FI. constructor; auto.
-  - intros.
+    intros.
     eapply stack_inject_aux_invariant; eauto.
-  - intros. eauto.
 Qed.
-
-  (* Lemma stack_inject_invariant': *)
-  (*   forall (m m': perm_type) f g f1 f2 thr, *)
-  (*     (forall b ofs k p, *)
-  (*         Plt b thr -> *)
-  (*         m' b ofs k p -> m b ofs k p) -> *)
-  (*     Forall (fun f1 => forall b, in_frames f1 b -> Plt b thr) f1 -> *)
-  (*     Forall (fun t1 => forall f1 b, In f1 (snd t1) -> in_frame f1 b -> Plt b thr) f1 -> *)
-  (*     (forall b1 b2 delta, f b1 = Some (b2, delta) -> *)
-  (*                     in_stack f2 b2 -> *)
-  (*                     Plt b1 thr) -> *)
-  (*     stack_inject f g m f1 f2 -> *)
-  (*     stack_inject f g m' f1 f2. *)
-  (* Proof. *)
-  (*   intros. *)
-  (*   eapply stack_inject_invariant; eauto. *)
-  (*   intros. *)
-  (*   elim H5. eapply H2; eauto. *)
-  (*   eapply in_stack'_in_stack; eauto. *)
-  (* Qed. *)
 
   Lemma stack_inject_aux_invariant_strong:
     forall (m m': perm_type) f g s1 s2,
-      stack_inject_aux f m g s1 s2 ->
+      stack_inject f m g s1 s2 ->
       (forall b ofs k p b' delta,
           f b = Some (b', delta) ->
           m' b ofs k p -> m b ofs k p) ->
-      stack_inject_aux f m' g s1 s2.
+      stack_inject f m' g s1 s2.
   Proof.
     induction 1; simpl; intros PERM; econstructor; eauto.
     eapply Forall_impl. 2: apply FI.
@@ -2089,25 +1680,23 @@ Qed.
     intros; eapply tframe_inject_invariant_strong; eauto.
   Qed.
 
+  (* used in Memory *)
   Lemma stack_inject_invariant_strong:
-    forall (m m': block -> _ -> _ -> _ -> Prop) f g f1 f2,
+    forall (m m': perm_type) f g f1 f2,
       (forall b ofs k p b' delta,
           f b = Some (b', delta) ->
           m' b ofs k p -> m b ofs k p) ->
-      stack_inject f g m f1 f2 ->
-      stack_inject f g m' f1 f2.
+      stack_inject f m  g f1 f2 ->
+      stack_inject f m' g f1 f2.
   Proof.
-    intros m m' f g f1 f2 PERM FI.
-    destruct FI. constructor; auto.
-    - intros. eapply stack_inject_aux_invariant_strong; eauto.
-    - intros; eapply stack_inject_not_in_source0; eauto.
+    intros. eapply stack_inject_aux_invariant_strong; eauto.
   Qed.
 
   Lemma stack_inject_nil:
     forall f p,
-      stack_inject f nil p nil nil.
+      stack_inject f p nil nil nil.
   Proof.
-    repeat constructor. easy.
+    repeat constructor.
   Qed.
 
   Lemma stack_inject_length_stack:
@@ -2116,12 +1705,11 @@ Qed.
       (length s2 <= length s1)%nat.
   Proof.
     intros j g P s1 s2 SI.
-    inversion SI.
-    revert stack_inject_frame_inject0. clear.
+    revert SI. clear.
     revert g s1 s2.
     induction 1; simpl; intros; eauto.
     simpl in *. repeat destr_in TAKE. simpl.
-    simpl in *. apply le_n_S. etransitivity. apply IHstack_inject_frame_inject0.
+    simpl in *. apply le_n_S. etransitivity. apply IHSI.
     rewrite drop_length. omega.
     eapply take_succeeds_inv; eauto.
   Qed.
@@ -2258,8 +1846,8 @@ Proof.
 Qed.
 
 Lemma size_frames_pos:
-  forall s,
-    (0 <= size_frames s)%Z.
+  forall tf,
+    (0 <= size_frames tf)%Z.
 Proof.
   intros. unfold size_frames. 
   apply Z.max_le_iff.
@@ -2362,7 +1950,7 @@ Qed.
 
   Lemma stack_inject_aux_id:
     forall p s,
-      stack_inject_aux inject_id p (flat_frameinj (length s)) s s.
+      stack_inject inject_id p (flat_frameinj (length s)) s s.
   Proof.
     induction s; simpl; intros; econstructor; simpl; eauto.
     repeat constructor.
@@ -2378,12 +1966,10 @@ Qed.
   Lemma stack_inject_id:
     forall p s,
       wf_stack p s ->
-      stack_inject inject_id (flat_frameinj (length s)) p s s.
+      stack_inject inject_id p (flat_frameinj (length s)) s s.
   Proof.
-    intros p s WF; constructor; auto.
+    intros p s WF; auto.
     eapply stack_inject_aux_id; eauto.
-    intros b1 b2 delta bi2 FB NIS FI o k p0 PERM IPC.
-    apply in_stack'_in_stack in FI. inv FB. congruence.
   Qed.
 
 (** The following shows how to transport a stack injection when more blocks get
@@ -2408,18 +1994,18 @@ allocated. *)
   Qed.
 
 Lemma stack_inject_aux_incr:
-  forall f f' g (p: block -> Z -> perm_kind -> permission -> Prop)  s1 s2,
-    stack_inject_aux f p g s1 s2 ->
+  forall f f' g (p: perm_type)  s1 s2,
+    stack_inject f p g s1 s2 ->
     inject_incr f f' ->
     (forall b b' delta,
         f b = None ->
         f' b = Some (b', delta) ->
         ~ in_stack s1 b) ->
-    stack_inject_aux f' p g s1 s2.
+    stack_inject f' p g s1 s2.
 Proof.
   induction 1; simpl; intros INCR NEW; econstructor; eauto.
   subst.
-  eapply IHstack_inject_aux; eauto.
+  eapply IHstack_inject; eauto.
   intros b b' delta H0 H1 INS. eapply NEW; eauto using in_stack_drop.
   eapply Forall_impl. 2: apply FI.
   simpl; intros.
@@ -2430,30 +2016,17 @@ Proof.
 Qed.
 
 Lemma stack_inject_incr:
-  forall f f' g (p: block -> Z -> perm_kind -> permission -> Prop)  s1 s2,
+  forall f f' g (p: perm_type)  s1 s2,
     inject_incr f f' ->
     (forall b b' delta,
         f b = None ->
         f' b = Some (b', delta) ->
-        ~ in_stack s1 b 
-        /\ forall fi,
-            in_stack' s2 (b', fi) ->
-            forall o k pp,
-              p b o k pp ->
-              inject_perm_condition pp ->
-              frame_public fi (o + delta)) ->
-    stack_inject f g p s1 s2 ->
-    stack_inject f' g p s1 s2.
+        ~ in_stack s1 b) ->
+    stack_inject f  p g s1 s2 ->
+    stack_inject f' p g s1 s2.
 Proof.
   intros f f' g p s1 s2 INCR NEW SI.
-  inversion SI; constructor; eauto.
-  - eapply stack_inject_aux_incr; eauto.
-    intros; eapply NEW; eauto.
-  - intros b1 b2 delta bi2 SOME NIS INS o k p0 P IPC.
-    destruct (f b1) as [[b2' delta']|] eqn:FB.
-    exploit INCR. eauto. rewrite SOME. inversion 1; subst.
-    eauto.
-    generalize (NEW _ _ _ FB SOME). intros (NIN1 & NIN2). eapply NIN2 in INS; eauto.
+  eapply stack_inject_aux_incr; eauto.
 Qed.
 
 Lemma norepet_1:
@@ -2480,12 +2053,12 @@ Definition make_singleton_frame_adt' (b: block) fi (sz: Z) :=
   |}.
 
   Lemma val_inject_ext:
-    forall j1 j2 m1 m2,
-      Val.inject j1 m1 m2 ->
+    forall j1 j2 v1 v2,
+      Val.inject j1 v1 v2 ->
       (forall x, j1 x = j2 x) ->
-      Val.inject j2 m1 m2.
+      Val.inject j2 v1 v2.
   Proof.
-    intros j1 j2 m1 m2 INJ EXT.
+    intros j1 j2 v1 v2 INJ EXT.
     inv INJ; econstructor; eauto.
     rewrite <- EXT; eauto.
   Qed.
@@ -2500,9 +2073,6 @@ Definition make_singleton_frame_adt' (b: block) fi (sz: Z) :=
     inv INJ; constructor; auto.
     eapply val_inject_ext; eauto.
   Qed.
-
-
-
 
 Lemma frame_inject_ext:
   forall j1 j2 f1 f2,
@@ -2523,7 +2093,7 @@ Lemma has_perm_frame_ext:
     has_perm_frame P j f ->
     has_perm_frame P j' f.
 Proof.
-  intros j j' P f EXT (b & o & k & p0 & FSOME & INFR1 & PERM & IPC).
+  intros j j' P f EXT (b & o & k & p0 & FSOME & INFR1 & PERM).
   repeat eexists; eauto. rewrite EXT in FSOME; auto.
 Qed.
 
@@ -2541,9 +2111,9 @@ Qed.
 
   Lemma stack_inject_aux_ext':
     forall j1 j2 g P m1 m2,
-      stack_inject_aux j1 P g m1 m2 ->
-      (forall x, j1 x = j2 x) ->
-      stack_inject_aux j2 P g m1 m2.
+      stack_inject j1 P g m1 m2 ->
+      (forall b, j1 b = j2 b) ->
+      stack_inject j2 P g m1 m2.
   Proof.
     induction 1; simpl; intros; econstructor; eauto.
     eapply Forall_impl. 2: apply FI.
@@ -2553,25 +2123,22 @@ Qed.
 
   Lemma stack_inject_ext':
     forall j1 j2 g P m1 m2,
-      stack_inject j1 g P m1 m2 ->
-      (forall x, j1 x = j2 x) ->
-      stack_inject j2 g P m1 m2.
+      stack_inject j1 P g m1 m2 ->
+      (forall b, j1 b = j2 b) ->
+      stack_inject j2 P g m1 m2.
   Proof.
     intros j1 j2 g P m1 m2 INJ EXT.
-    inv INJ; constructor; eauto.
-    - eapply stack_inject_aux_ext'; eauto.
-    - intros.
-      eapply stack_inject_not_in_source0; eauto. rewrite EXT; eauto.
+    eapply stack_inject_aux_ext'; eauto.
   Qed.
 
 
-    Lemma frameinj_push_flat:
-      forall m,
-        flat_frameinj (Datatypes.S m) = 1%nat :: flat_frameinj m.
-    Proof.
-      reflexivity.
-    Qed.
-    
+  Lemma frameinj_push_flat:
+    forall m,
+      flat_frameinj (Datatypes.S m) = 1%nat :: flat_frameinj m.
+  Proof.
+    reflexivity.
+  Qed.
+
 Lemma frame_at_pos_cons:
   forall l i f a,
     frame_at_pos l i f ->
@@ -2621,7 +2188,7 @@ Proof.
         simpl in *; auto.
 Qed.
 
-Open Scope nat_scope.
+Local Open Scope nat_scope.
 
 
 
@@ -2632,34 +2199,34 @@ Inductive top_tframe_prop (P: tframe_adt -> Prop) : stack -> Prop :=
     P tf ->
     top_tframe_prop P (tf::r).
 
-
-(* Definition wf_tframe_strong (m: perm_type) (j: meminj) (f: tframe_adt) : Prop := *)
-(*   forall b, *)
-(*     j b <> None -> *)
-(*     in_frames f b -> *)
-(*     forall o k p, ~ m b o k p. *)
-
-
 Definition top_tframe_tc (s: stack) : Prop :=
   top_tframe_prop (fun tf => fst tf = None) s.
 
+Lemma check_top_tc s : { top_tframe_tc s } + { ~ top_tframe_tc s }.
+Proof.
+  unfold top_tframe_tc.
+  destruct s eqn:STK. right; intro A; inv A.
+  destruct t.
+  destruct o.
+  right. intro A. inv A. inv H0.
+  left; constructor. auto.
+Defined.
+
 Lemma stack_inject_push_new_stage_right:
   forall j n g P s1 s2,
-    stack_inject j (n :: g) P s1 s2 ->
+    stack_inject j P (n :: g) s1 s2 ->
     top_tframe_tc s1 ->
     (2 <= n)%nat ->
-    stack_inject j (1%nat :: pred n :: g) P s1 ((None,nil)::s2).
+    stack_inject j P (1%nat :: pred n :: g) s1 ((None,nil)::s2).
 Proof.
   intros j n g P s1 s2 SI TTNP Gof1.
-  inversion SI; constructor; auto.
-  - inv stack_inject_frame_inject0.
-    simpl in *. repeat destr_in TAKE.
-    econstructor. reflexivity. simpl. eauto.
-    destruct n0. omega. econstructor; eauto. inv FI; auto.
-    repeat constructor.
-    intros ff1 INf1 _. exfalso.
-    inv TTNP. congruence.
-  - simpl. intros; eapply stack_inject_not_in_source0; eauto. tauto.
+  inv SI.
+  simpl in *. repeat destr_in TAKE.
+  econstructor. reflexivity. simpl. eauto.
+  destruct n0. omega. econstructor; eauto. inv FI; auto.
+  repeat constructor.
+  intros ff1 INf1 _. exfalso.
+  inv TTNP. congruence.
 Qed.
 
 Lemma frame_at_pos_cons_inv:
@@ -2675,38 +2242,27 @@ Qed.
 
 Lemma stack_inject_unrecord_parallel:
   forall j g m1 s1 s2
-    (SI: stack_inject j (1%nat :: g) m1 s1 s2)
+    (SI: stack_inject j m1 (1%nat :: g) s1 s2)
     (ND2: nodup s2)
     fr2 l2
     (STK2 : s2 = fr2 :: l2)
     fr1 l1
     (STK1 : s1 = fr1 :: l1),
-    stack_inject j g m1 l1 l2.
+    stack_inject j m1 g l1 l2.
 Proof.
   intros. subst.
-  inversion SI; constructor; auto.
-  + inv stack_inject_frame_inject0. simpl in *; auto.
-  + simpl. intros b1 b2 delta bi2 JB NIS INS o k p PERM IPC.
-    inv stack_inject_frame_inject0. simpl in *; auto. inv TAKE.
-    inv FI. clear H2.
-    destruct (in_frames_dec fr1 b1).
-    * destruct (in_frames_in_frame_ex _ _ i) as (fr & INfrs & INFR).
-      inv ND2. edestruct H3.
-      eapply tframe_inject_in_frames; eauto.
-      eapply in_stack'_in_stack; eauto.
-    * eapply stack_inject_not_in_source0 in JB; eauto.
-      rewrite in_stack_cons. intuition.
+  inv SI. simpl in *; auto.
 Qed.
 
 Lemma stack_inject_unrecord_parallel_frameinj_flat_on:
   forall j m1 s1 s2
-    (SI: stack_inject j (flat_frameinj (length s2)) m1 s1 s2)
+    (SI: stack_inject j m1 (flat_frameinj (length s2)) s1 s2)
     (ND2: nodup s2)
     fr2 l2
     (STK2 : s2 = fr2 :: l2)
     fr1 l1
     (STK1 : s1 = fr1 :: l1),
-    stack_inject j (flat_frameinj (length l2)) m1 l1 l2.
+    stack_inject j m1 (flat_frameinj (length l2)) l1 l2.
 Proof.
   intros. subst.
   eapply stack_inject_unrecord_parallel; eauto.
@@ -2719,7 +2275,7 @@ Lemma same_sizes_frame_size_eq:
     same_sizes_frame f1 f2 ->
     size_frame f1 = size_frame f2.
 Proof.
-  intros f1 f2 SS; unfold size_frame; rewrite SS. reflexivity.
+  intros f1 f2 SS; unfold size_frame. rewrite SS. reflexivity.
 Qed.
 
 Definition same_sizes_list_frames tf1 tf2 :=
@@ -2821,91 +2377,14 @@ Proof.
 Qed.
 End INJ.
 
-Program Definition inject_perm_upto_writable: InjectPerm :=
-  {|
-    inject_perm_condition := fun p => perm_order Writable p
-  |}.
-
-Program Definition inject_perm_all: InjectPerm :=
-  {|
-    inject_perm_condition := fun p => True
-  |}.
-
-(* Definition same_head (P: perm_type) (m m': stack) := *)
-(*   list_forall2 *)
-(*     (fun tf1 tf2 => *)
-(*        (forall f1, In f1 tf1 -> has_perm_frame (injperm:=inject_perm_all) P inject_id f1 -> In f1 tf2) *)
-(*        /\ (forall f1, In f1 tf2 -> In f1 tf1) *)
-(*     ) *)
-(*     m m'. *)
-
-(* Lemma same_head_in_stack': *)
-(*   forall P s1 s2, same_head P s1 s2 -> forall b fi, in_stack' s2 (b,fi) -> in_stack' s1 (b,fi). *)
-(* Proof. *)
-(*   induction 1; simpl; intros; eauto. *)
-(*   destruct H. *)
-(*   destruct H1; auto. *)
-(*   left. *)
-(*   rewrite in_frames'_rew in H1. destruct H1 as (fr & IFR & INb1). *)
-(*   apply H2 in INb1. *)
-(*   rewrite in_frames'_rew; eauto. *)
-(* Qed. *)
-
-(* Lemma same_head_get_frame_info: *)
-(*   forall P s1 s2 (SH: same_head P s1 s2) *)
-(*     (ND: nodup s1) (ND': Forall nodupt s1) *)
-(*     b f (GFI: get_frame_info s2 b = Some f), *)
-(*     get_frame_info s1 b = Some f. *)
-(* Proof. *)
-(*   intros. *)
-(*   apply get_assoc_spec in GFI. *)
-(*   destruct GFI as (fr & tf & INblocks & INtf & INS). *)
-(*   exploit same_head_in_stack'; eauto. *)
-(*   rewrite in_stack'_rew. eexists; split; eauto. *)
-(*   rewrite in_frames'_rew. eexists; split; eauto. *)
-(*   intro INS'. *)
-(*   clear INblocks INtf INS. *)
-(*   rewrite in_stack'_rew in INS'. setoid_rewrite in_frames'_rew in INS'. *)
-(*   destruct INS' as (ttf & (tfr & IFR & ITF) & INS). *)
-(*   eapply get_assoc_stack_lnr; eauto. *)
-(* Qed. *)
-
-(* Lemma same_head_in_impl: *)
-(*   forall P s1 s2, same_head P s1 s2 -> forall b, in_stack s2 b -> in_stack s1 b. *)
-(* Proof. *)
-(*   intros. *)
-(*   eapply in_stack_in_frames_ex in H0. destruct H0 as (tf & INS & IFRS). *)
-(*   eapply in_frames_in_frame_ex in IFRS. destruct IFRS as (fr & IFRS & IFR). *)
-(*   apply in_frame_info in IFR. destruct IFR as (fi & IFR). *)
-(*   eapply in_stack'_in_stack. eapply same_head_in_stack'; eauto. *)
-(*   rewrite in_stack'_rew. eexists; split; eauto. *)
-(*   rewrite in_frames'_rew. eexists; split; eauto. *)
-(* Qed. *)
-
-(* Lemma same_head_fap: *)
-(*   forall P s1 s2 (SH: same_head P s1 s2) *)
-(*          f1 i (FAP1: f1 @ s1 : i), *)
-(*   exists f2, f2 @ s2 : i /\ (forall ff1, In ff1 f1 -> has_perm_frame (injperm:= inject_perm_all) P inject_id ff1 -> In ff1 f2). *)
-(* Proof. *)
-(*   induction 1; simpl; intros; eauto. *)
-(*   destruct H. *)
-(*   destruct i. *)
-(*   - apply frame_at_pos_last in FAP1. subst. *)
-(*     exists b1; split. constructor; reflexivity. *)
-(*     auto. *)
-(*   - apply frame_at_pos_cons_inv in FAP1. *)
-(*     eapply IHSH in FAP1. destruct FAP1 as (f2 & FAP2 & PROP). *)
-(*     exists f2; split. apply frame_at_pos_cons. auto. eauto. omega. *)
-(* Qed. *)
-
-Lemma has_perm_frame_impl {injperm: InjectPerm}:
+Lemma has_perm_frame_impl:
   forall (P1 P2: perm_type) j f tf,
     has_perm_frame P1 j f ->
     frame_inject j f tf ->
-    (forall b1 b2 delta o k p, j b1 = Some (b2, delta) -> P1 b1 o k p -> inject_perm_condition p -> P2 b2 (o + delta)%Z k p) ->
+    (forall b1 b2 delta o k p, j b1 = Some (b2, delta) -> P1 b1 o k p -> P2 b2 (o + delta)%Z k p) ->
     has_perm_frame P2 inject_id tf.
 Proof.
-  intros P1 P2 j f tf (b & o & k & p & NONE & IFR & PERM1 & IPC) FI PERMS.
+  intros P1 P2 j f tf (b & o & k & p & NONE & IFR & PERM1) FI PERMS.
   red in FI.
   apply in_frame_info in IFR. destruct IFR as (fi & IFR).
   rewrite Forall_forall in FI; specialize (FI _ IFR).
@@ -2914,83 +2393,11 @@ Proof.
   specialize (FI _ _ eq_refl).
   destruct FI as (fi' & IN' & IFI).
   exists b0, (o + z)%Z, k, p. split. unfold inject_id. congruence.
-  split. eapply in_frame'_in_frame; eauto. split; eauto.
+  split. eapply in_frame'_in_frame; eauto. eauto.
 Qed.
-
-(* Lemma same_head_more_perm {injperm: InjectPerm}: *)
-(*   forall (P1 P2: perm_type) s1 s2 *)
-(*          (SH: same_head P1 s1 s2) *)
-(*          (SAMEPERM: forall b o k p, in_stack s1 b -> P2 b o k p -> P1 b o k p), *)
-(*     same_head P2 s1 s2. *)
-(* Proof. *)
-(*   induction 1; simpl; intros; constructor; auto. *)
-(*   - destruct H; split; auto. *)
-(*     intros; eapply H; eauto. *)
-(*     destruct H2 as (b & o & k & p & NONE & IFR & PERM & IPC). *)
-(*     exists b, o, k, p; repeat split; eauto. eapply SAMEPERM; eauto. *)
-(*     rewrite in_stack_cons; left. *)
-(*     eapply in_frame_in_frames; eauto. *)
-(*   - apply IHSH. intros. eapply SAMEPERM; eauto. *)
-(*     apply in_stack_tl. simpl; auto. *)
-(* Qed. *)
-
-(* Lemma public_stack_access_same_head: *)
-(*   forall s1 (ND: nodup s1) (ND': Forall nodupt s1) s2 P (SH: same_head P s1 s2) b lo hi *)
-(*          (PSA: public_stack_access s1 b lo hi), *)
-(*     public_stack_access s2 b lo hi. *)
-(* Proof. *)
-(*   intros. red. destr. red in PSA. *)
-(*   erewrite same_head_get_frame_info in PSA; eauto. *)
-(* Qed. *)
 
 Definition stack_top_is_new s :=
   top_tframe_prop (fun tf => tf = (None,nil)) s.
-
-(* Lemma is_stack_top_same_head: *)
-(*   forall P s1 (WF: wf_stack P inject_id s1) (ND: nodup s1) s2 (SH: same_head P s1 s2) b *)
-(*          o k p (PERM: P b o k p) *)
-(*          (IST: is_stack_top s1 b), *)
-(*     is_stack_top s2 b \/ ~ in_stack s2 b. *)
-(* Proof. *)
-(*   intros. *)
-(*   inv SH. easy. *)
-(*   destruct H. *)
-(*   red in IST. simpl in IST. *)
-(*   change (in_frames a1 b) in IST. *)
-(*   left. red. simpl. *)
-(*   change (in_frames b1 b). *)
-(*   edestruct in_frames_in_frame_ex as (fr & IFRS & IFR). eauto. *)
-(*   eapply in_frame_in_frames; eauto. apply H; auto. *)
-(*   exists b, o, k, p; repeat split; auto. unfold inject_id; congruence. *)
-(* Qed. *)
-
-(* Lemma stack_access_same_head: *)
-(*   forall s1 P (ND: nodup s1) (ND': Forall nodupt s1) (WF: wf_stack P inject_id s1) s2 (SH: same_head P s1 s2) b lo hi k p *)
-(*          (R: forall o, (lo <= o < hi)%Z -> P b o k p) *)
-(*          (SA: stack_access s1 b lo hi), *)
-(*     stack_access s2 b lo hi. *)
-(* Proof. *)
-(*   intros. *)
-(*   destruct (zlt lo hi). *)
-(*   destruct SA as [IST|PSA]. *)
-(*   edestruct is_stack_top_same_head; eauto. apply (R lo). omega. left; auto. *)
-(*   right; red; destr. eapply get_frame_info_in_stack in Heqo; congruence. *)
-(*   right; eapply public_stack_access_same_head; eauto. *)
-(*   eapply lo_ge_hi_stack_access; eauto. *)
-(* Qed. *)
-
-(* Lemma stack_access_same_head_or_not_in_stack: *)
-(*   forall s1 P (ND: nodup s1) (ND': Forall nodupt s1) (WF: wf_stack P inject_id s1) s2 b *)
-(*          (SH: same_head P s1 s2 \/ ~ in_stack s2 b) lo hi k p *)
-(*          (R: forall o, (lo <= o < hi)%Z -> P b o k p) *)
-(*          (SA: stack_access s1 b lo hi), *)
-(*     stack_access s2 b lo hi. *)
-(* Proof. *)
-(*   intros. *)
-(*   destruct SH as [SH | NIS]. *)
-(*   eapply stack_access_same_head; eauto. *)
-(*   right. red. destr. apply get_frame_info_in_stack in Heqo. congruence.           *)
-(* Qed. *)
 
 Lemma max_in_le:
   forall l a i,
@@ -3014,24 +2421,6 @@ Proof.
   apply max_in_le; auto.
   apply IHl1. auto.
 Qed.
-
-(* Lemma same_head_size: *)
-(*   forall P s1 s2, *)
-(*     same_head P s1 s2 -> *)
-(*     (size_stack s2 <= size_stack s1)%Z. *)
-(* Proof. *)
-(*   induction 1; simpl; intros; rewrite ? size_stack_cons. omega. *)
-(*   cut (size_frames b1 <= size_frames a1)%Z. omega. *)
-(*   apply max_sublist. setoid_rewrite in_map_iff. *)
-(*   intros x (x0 & EQ & IN). exists x0; split; auto. apply H. auto. *)
-(* Qed. *)
-
-(* Lemma same_head_refl: *)
-(*   forall P s, *)
-(*     same_head P s s. *)
-(* Proof. *)
-(*   induction s; simpl; intros; constructor; eauto. *)
-(* Qed. *)
 
 (* For use in Mach and Asm, the parent_sp pointer is now computed on the stack
    adt rather than on the abstract semantic callstack in Mach or with an extra
@@ -3066,6 +2455,7 @@ Proof.
   unfold parent_sp, current_sp, current_frame_sp. intros.
   repeat destr; try now (simpl; auto).
 Qed.
+
 Definition opt_cons {A: Type} (o: option A) (l: list A) : list A :=
   match o with
     None => l
@@ -3119,3 +2509,420 @@ Proof.
   apply size_frame_pos. omega.    
 Qed.
 
+(* (** SACC: The following property is needed by ValueDomain, to prove mmatch_inj. *)
+Definition record_init_sp m :=
+  let (m1, b1) := alloc (push_new_stage m) 0 0 in
+  record_stack_blocks m1 (make_singleton_frame_adt b1 0 0). 
+
+  Lemma record_init_sp_inject:
+    forall j g m1 m1' m2,
+      Mem.inject j g m1 m1' ->
+      size_stack (stack m1') <= size_stack (stack m1) ->
+      record_init_sp m1 = Some m2 ->
+      exists m2', record_init_sp m1' = Some m2' /\ inject (fun b => if peq b (nextblock (push_new_stage m1))
+                                                           then Some (nextblock (push_new_stage m1'), 0)
+                                                           else j b) (1%nat::g) m2 m2'.
+  Proof.
+    intros j g m1 m1' m2 INJ SZ RIS.
+    unfold record_init_sp in *; destr_in RIS.
+    exploit Mem.push_new_stage_inject. apply INJ. intro INJ0.
+    edestruct Mem.alloc_parallel_inject as (f' & m2' & b2 & ALLOC & INJ1 & INCR & JNEW & JOLD).
+    apply INJ0. eauto. reflexivity. reflexivity.
+    rewrite ALLOC.
+    edestruct record_push_inject_alloc as (m2'' & RSB & INJ'). 7: apply RIS.
+    2: apply Heqp. 2: apply ALLOC. all: eauto.
+    rewrite push_new_stage_stack. constructor; reflexivity.
+    rewrite ! push_new_stage_stack. simpl. auto.
+    eexists; split. eauto.
+    eapply inject_ext. eauto.
+    intros. erewrite <- ! alloc_result by eauto.
+    destr. eauto.
+  Qed.
+
+  Lemma record_init_sp_extends:
+    forall m1 m1' m2,
+      Mem.extends m1 m1' ->
+      size_stack (stack m1') <= size_stack (stack m1) ->
+      record_init_sp m1 = Some m2 ->
+      exists m2', record_init_sp m1' = Some m2' /\ extends m2 m2'.
+  Proof.
+    intros m1 m1' m2 INJ SZ RIS.
+    unfold record_init_sp in *; destr_in RIS.
+    apply extends_push in INJ.
+    edestruct alloc_extends as (m2' & ALLOC & INJ1).
+    apply INJ. eauto. reflexivity. reflexivity.
+    rewrite ALLOC.
+    edestruct record_push_extends_flat_alloc as (m2'' & RSB & INJ'). 4: apply RIS.
+    apply Heqp. apply ALLOC. all: eauto.
+    rewrite push_new_stage_stack. constructor; reflexivity.
+    rewrite ! push_new_stage_stack. simpl. auto.
+  Qed.
+
+  Lemma record_init_sp_flat_inject
+    : forall (m1 m1' m2 : mem),
+      Mem.inject (Mem.flat_inj (Mem.nextblock m1)) (flat_frameinj (length (Mem.stack m1))) m1 m1' ->
+      size_stack (Mem.stack m1') <= size_stack (Mem.stack m1) ->
+      Mem.record_init_sp m1 = Some m2 ->
+      Mem.nextblock m1 = Mem.nextblock m1' ->
+      exists m2' : mem,
+        Mem.record_init_sp m1' = Some m2' /\
+        Mem.inject
+          (Mem.flat_inj (Mem.nextblock m2))
+          (flat_frameinj (length (Mem.stack m2))) m2 m2'.
+  Proof.
+    intros m1 m1' m2 INJ SZ RIS EQNB.
+    edestruct record_init_sp_inject as (m2' & RIS' & INJ'); eauto.
+    eexists; split; eauto.
+    unfold record_init_sp in RIS; destr_in RIS.
+    erewrite (record_stack_block_nextblock _ _ _ RIS).
+    erewrite (nextblock_alloc _ _ _ _ _ Heqp).
+    rewrite push_new_stage_nextblock.
+    destruct (record_stack_blocks_stack_eq _ _ _ RIS) as (tf & r & EQ1 & EQ2).
+    rewrite EQ2. 
+    erewrite (alloc_stack_blocks _ _ _ _ _ Heqp) in EQ1.
+    rewrite push_new_stage_stack in EQ1. inv EQ1.
+    simpl. rewrite frameinj_push_flat.
+    eapply inject_ext; eauto.
+    simpl; intros. unfold flat_inj.
+    rewrite ! push_new_stage_nextblock. rewrite EQNB.
+    repeat (destr; subst); xomega.
+  Qed.
+
+  Lemma record_init_sp_nextblock:
+    forall m1 m2,
+      record_init_sp m1 = Some m2 ->
+      Ple (nextblock m1) (nextblock m2).
+  Proof.
+    intros m1 m2 RIS.
+    unfold record_init_sp in RIS. destr_in RIS.
+    erewrite (record_stack_block_nextblock _ _ _ RIS).
+    erewrite (nextblock_alloc _ _ _ _ _ Heqp).
+    rewrite push_new_stage_nextblock. xomega.
+  Qed.
+
+  Lemma record_init_sp_nextblock_eq:
+    forall m1 m2,
+      record_init_sp m1 = Some m2 ->
+      (nextblock m2) = Pos.succ (nextblock m1).
+  Proof.
+    intros m1 m2 RIS.
+    unfold record_init_sp in RIS. destr_in RIS.
+    erewrite (record_stack_block_nextblock _ _ _ RIS).
+    erewrite (nextblock_alloc _ _ _ _ _ Heqp).
+    rewrite push_new_stage_nextblock. reflexivity.
+  Qed.
+  
+  Lemma record_init_sp_stack:
+    forall m1 m2,
+      Mem.record_init_sp m1 = Some m2 ->
+      Mem.stack m2 = (Some (make_singleton_frame_adt (Mem.nextblock (Mem.push_new_stage m1)) 0 0),nil)::Mem.stack m1.
+  Proof.
+    unfold Mem.record_init_sp. intros m1 m2 RIS; destr_in RIS.
+    destruct (record_stack_blocks_stack_eq _ _ _ RIS) as (tf & r & EQ1 & EQ2).
+    rewrite EQ2. 
+    erewrite (alloc_stack_blocks _ _ _ _ _ Heqp) in EQ1.
+    rewrite push_new_stage_stack in EQ1. inv EQ1.
+    exploit Mem.alloc_result; eauto. intros; subst. reflexivity.
+  Qed.
+  
+  Lemma record_init_sp_perm:
+    forall m1 m2,
+      Mem.record_init_sp m1 = Some m2 ->
+      forall b o k p,
+        perm m2 b o k p <-> perm m1 b o k p.
+  Proof.
+    unfold Mem.record_init_sp. intros m1 m2 RIS; destr_in RIS.
+    intros.
+    split; intro P.
+    - eapply push_new_stage_perm.
+      eapply record_stack_block_perm in P. 2: eauto.
+      eapply perm_alloc_inv in P; eauto.
+      destr_in P. omega.
+    - eapply record_stack_block_perm'. eauto.
+      eapply perm_alloc_1. eauto.
+      eapply push_new_stage_perm. auto.
+  Qed.
+*)
+
+(*   Definition is_ptr (v: val) :=
+    match v with Vptr _ _ => Some v | _ => None end.
+  
+  Definition encoded_ra (l: list memval) : option val :=
+    match proj_bytes l with
+    | Some bl => Some (Vptrofs (Ptrofs.repr (decode_int bl)))
+    | None => is_ptr (Val.load_result Mptr (proj_value (quantity_chunk Mptr) l))
+    end.
+
+  Definition loadbytesv chunk m addr :=
+    match addr with
+      Vptr b o =>
+      match Mem.loadbytes m b (Ptrofs.unsigned o) (size_chunk chunk) with
+      | Some bytes => encoded_ra bytes
+      | None => None
+      end
+    | _ => None
+    end.
+
+  Lemma loadbytesv_inject:
+    forall j g chunk m m' v v' ra,
+      Mem.inject j g m m' ->
+      Val.inject j v v' ->
+      loadbytesv chunk m v = Some ra ->
+      exists ra', loadbytesv chunk m' v' = Some ra' /\ Val.inject j ra ra'.
+  Proof.
+    intros j g chunk m m' v v' ra MINJ VINJ L.
+    unfold loadbytesv in *.
+    destr_in L. inv VINJ.
+    destr_in L.
+    edestruct Mem.loadbytes_inject as (l' & L' & INJ); eauto.
+    erewrite Mem.address_inject; eauto.
+    rewrite L'.
+    - unfold encoded_ra in L |- *.
+      repeat destr_in L.
+      erewrite proj_bytes_inject; eauto.
+      destr. eapply proj_bytes_not_inject in Heqo0; eauto. 2: congruence.
+      erewrite proj_value_undef in H0; eauto.
+      contradict H0. unfold Mptr. destr; simpl; congruence.
+      generalize (proj_value_inject _ (quantity_chunk Mptr) _ _ INJ). intro VINJ.
+      generalize (Val.load_result_inject _ Mptr _ _ VINJ). intro VINJ'.
+      unfold is_ptr in H0. destr_in H0. inv H0. inv VINJ'.
+      eexists; split. simpl. eauto.
+      econstructor; eauto.
+    - eapply Mem.loadbytes_range_perm; eauto. generalize (size_chunk_pos chunk); omega.
+  Qed.
+
+  Lemma loadbytesv_extends:
+    forall chunk m m' v v' ra,
+      Mem.extends m m' ->
+      Val.lessdef v v' ->
+      loadbytesv chunk m v = Some ra ->
+      exists ra', loadbytesv chunk m' v' = Some ra' /\ Val.lessdef ra ra'.
+  Proof.
+    intros chunk m m' v v' ra MEXT VLD L.
+    unfold loadbytesv in *.
+    destr_in L. inv VLD.
+    destr_in L.
+    edestruct Mem.loadbytes_extends as (l' & L' & EXT); eauto.
+    rewrite L'.
+    - unfold encoded_ra in L |- *.
+      repeat destr_in L.
+      erewrite proj_bytes_inject; eauto.
+      destr. eapply proj_bytes_not_inject in Heqo0; eauto. 2: congruence.
+      erewrite proj_value_undef in H0; eauto.
+      contradict H0. unfold Mptr. destr; simpl; congruence.
+      generalize (proj_value_inject _ (quantity_chunk Mptr) _ _ EXT). intro VEXT.
+      generalize (Val.load_result_inject _ Mptr _ _ VEXT). intro VEXT'.
+      unfold is_ptr in H0. destr_in H0. inv H0. inv VEXT'. inv H2.
+      eexists; split. simpl. eauto.
+      rewrite Ptrofs.add_zero. econstructor; eauto.
+  Qed.
+
+  
+  Lemma proj_value_inj_value:
+    forall q v l,
+      proj_value q l = v ->
+      v <> Vundef ->
+      inj_value q v = l.
+  Proof.
+    unfold proj_value.
+    intros q v l PROJ NU.
+    subst. destr. destr. destr.
+    destruct q; simpl in Heqb;
+      repeat match goal with
+             | H: andb _ _ = true |- _ => rewrite andb_true_iff in H; destruct H
+             | H: proj_sumbool (quantity_eq ?q1 ?q2) = true |- _ =>
+               destruct (quantity_eq q1 q2); simpl in H; try congruence; subst
+             | H: proj_sumbool (Val.eq ?q1 ?q2) = true |- _ =>
+               destruct (Val.eq q1 q2); simpl in H; try congruence; subst
+             | H: context [match ?a with _ => _ end] |- _ => destruct a eqn:?; simpl in *; intuition try congruence
+             end.
+  Qed.
+
+  Lemma long_unsigned_ptrofs_repr_eq:
+    Archi.ptr64 = true -> forall a, Int64.unsigned (Ptrofs.to_int64 (Ptrofs.repr a)) = Ptrofs.unsigned (Ptrofs.repr a).
+  Proof.
+    intros.
+    unfold Ptrofs.to_int64.
+    rewrite <- Ptrofs.agree64_repr; auto.
+    rewrite Ptrofs.repr_unsigned. auto.
+  Qed.
+
+  Lemma int_unsigned_ptrofs_repr_eq:
+    Archi.ptr64 = false -> forall a, Int.unsigned (Ptrofs.to_int (Ptrofs.repr a)) = Ptrofs.unsigned (Ptrofs.repr a).
+  Proof.
+    intros.
+    unfold Ptrofs.to_int.
+    rewrite <- Ptrofs.agree32_repr; auto.
+    rewrite Ptrofs.repr_unsigned. auto.
+  Qed.
+
+  Lemma byte_decompose: forall i x, (Byte.unsigned i + x * 256) / 256 = x.
+  Proof.
+    intros.
+    rewrite Z_div_plus_full.
+    rewrite Zdiv_small. omega. apply Byte.unsigned_range. omega.
+  Qed.
+
+  Lemma ptrofs_wordsize: Ptrofs.zwordsize = 8 * size_chunk Mptr.
+  Proof.
+    unfold Ptrofs.zwordsize, Ptrofs.wordsize.
+    unfold Wordsize_Ptrofs.wordsize. unfold Mptr.
+    destr; omega.
+  Qed.
+  
+  Lemma ptrofs_byte_modulus_ptr64:
+    Archi.ptr64 = true ->
+    Byte.modulus ^ 8 - 1 = Ptrofs.max_unsigned.
+  Proof.
+    unfold Ptrofs.max_unsigned. rewrite Ptrofs.modulus_power.
+    rewrite ptrofs_wordsize.
+    intros. unfold Mptr; rewrite H. simpl. reflexivity.
+  Qed.
+
+  Lemma ptrofs_byte_modulus_ptr32:
+    Archi.ptr64 = false ->
+    Byte.modulus ^ 4 - 1 = Ptrofs.max_unsigned.
+  Proof.
+    unfold Ptrofs.max_unsigned. rewrite Ptrofs.modulus_power.
+    rewrite ptrofs_wordsize.
+    intros. unfold Mptr; rewrite H. simpl. reflexivity.
+  Qed.
+
+  Lemma byte_compose_range:
+    forall i x n,
+      0 < n ->
+      0 <= x < Byte.modulus ^ (n - 1) ->
+      0 <= Byte.unsigned i + x * 256 < Byte.modulus ^ n.
+  Proof.
+    intros i x n POS RNG.
+    split.
+    generalize (Byte.unsigned_range i). omega.
+    generalize (Byte.unsigned_range i). 
+    change Byte.modulus with 256 in *. 
+    replace n with ((n-1)+1) by omega. rewrite Zpower_exp by omega.
+    change (256 ^ 1) with 256.
+    assert (0 <= x * 256 < 256 ^ (n - 1) * 256).
+    split. omega.
+    apply Z.mul_lt_mono_pos_r. omega. omega.
+    omega.
+  Qed.
+
+  Lemma le_m1_lt:
+    forall a b,
+      0 <= a < b ->
+      0 <= a <= b - 1.
+  Proof.
+    intros; omega.
+  Qed.
+
+  Lemma byte_repr_plus i0 i:
+    Byte.repr (Byte.unsigned i0 + i * 256) = i0.
+  Proof.
+    apply Byte.eqm_repr_eq.
+    red. red. exists i.
+    change Byte.modulus with 256 in *. omega.
+  Qed.
+  
+  Lemma encode_decode_long:
+    forall l,
+      length l = 8%nat ->
+      Archi.ptr64 = true ->
+      encode_int 8 (Int64.unsigned (Ptrofs.to_int64 (Ptrofs.repr (decode_int l)))) = l.
+  Proof.
+    intros.
+    repeat match goal with
+           | H : length ?l = _ |- _ =>
+             destruct l; simpl in H; inv H
+           end. simpl.
+    unfold encode_int, decode_int.
+    unfold rev_if_be. destr.
+    - simpl.
+      rewrite Z.add_0_r.
+      rewrite ! long_unsigned_ptrofs_repr_eq; auto.
+      f_equal; rewrite ! Ptrofs.unsigned_repr.
+      rewrite ! byte_decompose; apply Byte.repr_unsigned.
+      rewrite <- ptrofs_byte_modulus_ptr64; auto.
+      apply le_m1_lt.
+      repeat (apply byte_compose_range; [omega |]).
+      simpl Z.sub. apply Byte.unsigned_range.
+      f_equal. rewrite ! byte_decompose. apply byte_repr_plus.
+      f_equal. rewrite ! byte_decompose. apply byte_repr_plus.
+      f_equal. rewrite ! byte_decompose. apply byte_repr_plus.
+      f_equal. rewrite ! byte_decompose. apply byte_repr_plus.
+      f_equal. rewrite ! byte_decompose. apply byte_repr_plus.
+      f_equal. rewrite ! byte_decompose. apply byte_repr_plus.
+      f_equal. apply byte_repr_plus.
+      rewrite <- ptrofs_byte_modulus_ptr64; auto.
+      apply le_m1_lt.
+      repeat (apply byte_compose_range; [omega |]).
+      simpl Z.sub. apply Byte.unsigned_range.
+    - simpl.
+      rewrite Z.add_0_r.
+      rewrite ! long_unsigned_ptrofs_repr_eq; auto.
+      f_equal; rewrite ! Ptrofs.unsigned_repr.
+      apply byte_repr_plus.
+      rewrite <- ptrofs_byte_modulus_ptr64; auto.
+      apply le_m1_lt.
+      repeat (apply byte_compose_range; [omega |]).
+      simpl Z.sub. apply Byte.unsigned_range.
+      f_equal. rewrite ! byte_decompose. apply byte_repr_plus.
+      f_equal. rewrite ! byte_decompose. apply byte_repr_plus.
+      f_equal. rewrite ! byte_decompose. apply byte_repr_plus.
+      f_equal. rewrite ! byte_decompose. apply byte_repr_plus.
+      f_equal. rewrite ! byte_decompose. apply byte_repr_plus.
+      f_equal. rewrite ! byte_decompose. apply byte_repr_plus.
+      f_equal. rewrite ! byte_decompose. apply Byte.repr_unsigned.
+      rewrite <- ptrofs_byte_modulus_ptr64; auto.
+      apply le_m1_lt.
+      repeat (apply byte_compose_range; [omega |]).
+      simpl Z.sub. apply Byte.unsigned_range.
+  Qed.
+
+  Lemma encode_decode_int:
+    forall l,
+      length l = 4%nat ->
+      Archi.ptr64 = false ->
+      encode_int 4 (Int.unsigned (Ptrofs.to_int (Ptrofs.repr (decode_int l)))) = l.
+  Proof.
+    intros.
+    repeat match goal with
+           | H : length ?l = _ |- _ =>
+             destruct l; simpl in H; inv H
+           end. simpl.
+    unfold encode_int, decode_int.
+    unfold rev_if_be. destr.
+    - simpl.
+      rewrite Z.add_0_r.
+      rewrite ! int_unsigned_ptrofs_repr_eq; auto.
+      f_equal; rewrite ! Ptrofs.unsigned_repr.
+      rewrite ! byte_decompose; apply Byte.repr_unsigned.
+      rewrite <- ptrofs_byte_modulus_ptr32; auto.
+      apply le_m1_lt.
+      repeat (apply byte_compose_range; [omega |]).
+      simpl Z.sub. apply Byte.unsigned_range.
+      f_equal. rewrite ! byte_decompose. apply byte_repr_plus.
+      f_equal. rewrite ! byte_decompose. apply byte_repr_plus.
+      f_equal. apply byte_repr_plus.
+      rewrite <- ptrofs_byte_modulus_ptr32; auto.
+      apply le_m1_lt.
+      repeat (apply byte_compose_range; [omega |]).
+      simpl Z.sub. apply Byte.unsigned_range.
+    - simpl.
+      rewrite Z.add_0_r.
+      rewrite ! int_unsigned_ptrofs_repr_eq; auto.
+      f_equal; rewrite ! Ptrofs.unsigned_repr.
+      apply byte_repr_plus.
+      rewrite <- ptrofs_byte_modulus_ptr32; auto.
+      apply le_m1_lt.
+      repeat (apply byte_compose_range; [omega |]).
+      simpl Z.sub. apply Byte.unsigned_range.
+      f_equal. rewrite ! byte_decompose. apply byte_repr_plus.
+      f_equal. rewrite ! byte_decompose. apply byte_repr_plus.
+      f_equal. rewrite ! byte_decompose. apply Byte.repr_unsigned.
+      rewrite <- ptrofs_byte_modulus_ptr32; auto.
+      apply le_m1_lt.
+      repeat (apply byte_compose_range; [omega |]).
+      simpl Z.sub. apply Byte.unsigned_range.
+  Qed.
+
+*)
